QVM/RZArith.v
@@ -4,6 +4,8 @@ Require Import SQIR.
 Require Import VectorStates UnitaryOps Coq.btauto.Btauto Coq.NArith.Nnat. 
 Require Import Dirac.
 Require Import QPE.
+Require Import BasicUtility.
+Require Import MathSpec.
 Require Import PQASM.
 Require Import CLArith.
 
@@ -55,41 +57,41 @@ Fixpoint rz_sub' (x:var) (n:nat) (size:nat) (M: nat -> bool) :=
 Definition rz_sub (x:var) (n:nat) (M:nat -> bool) := rz_sub' x n n M.
 
 Definition rz_compare_half (x:var) (n:nat) (c:posi) (M:nat) := 
-  Exp (rz_sub x n (nat2fb M)) ;; RQFT x ;; Exp (CNOT (x,0) c).
+   (rz_sub x n (nat2fb M)) ; RQFT x ; (CNOT (x,0) c).
 
 Definition rz_compare (x:var) (n:nat) (c:posi) (M:nat) := 
- rz_compare_half x n c M ;; (inv_pexp (Exp (rz_sub x n (nat2fb M)) ;; RQFT x)).
+ rz_compare_half x n c M ; (inv_exp ( (rz_sub x n (nat2fb M)) ; RQFT x)).
 
 Definition qft_cu (x:var) (c:posi) := 
-  RQFT x ;; Exp (CNOT (x,0) c) ;; QFT x.
+  RQFT x ;  (CNOT (x,0) c) ; QFT x.
 
 Definition qft_acu (x:var) (c:posi) := 
-  RQFT x ;; Exp (X (x,0); CNOT (x,0) c; X (x,0)) ;; QFT x.
+  RQFT x ;  (X (x,0); CNOT (x,0) c; X (x,0)) ; QFT x.
 
 Definition one_cu_adder (x:var) (n:nat) (c:posi) (M:nat -> bool) := CU c (rz_adder x n M).
 
 Definition mod_adder_half (x:var) (n:nat) (c:posi) (A:nat -> bool) (M:nat -> bool) :=
-  Exp (rz_adder x n A; (rz_sub x n M)) ;; qft_cu x c ;; Exp (one_cu_adder x n c M).
+   (rz_adder x n A; (rz_sub x n M)) ; qft_cu x c ;  (one_cu_adder x n c M).
 
 Definition clean_hbit (x:var) (n:nat) (c:posi) (M:nat -> bool) := 
-  Exp (rz_sub x n M) ;; qft_acu x c ;; Exp( inv_exp (rz_sub x n M)).
+   (rz_sub x n M) ; qft_acu x c ; ( inv_exp (rz_sub x n M)).
 
 Definition mod_adder (x:var) (n:nat) (c:posi) (A:nat -> bool) (M:nat -> bool) :=
-  mod_adder_half x n c A M ;; clean_hbit x n c A.
+  mod_adder_half x n c A M ; clean_hbit x n c A.
 
 (* modular multiplier: takes [x][0] -> [x][ax%N] where a and N are constant. *)
 Fixpoint rz_modmult' (y:var) (x:var) (n:nat) (size:nat) (c:posi) (A:nat) (M:nat) :=
    match n with
-   | 0 => Exp (SKIP (y,0))
-   | S m => rz_modmult' y x m size c A M;;
-           PCU (x,size - n) (mod_adder y size c (nat2fb ((2^m * A) mod M)) (nat2fb M))
+   | 0 =>  (SKIP (y,0))
+   | S m => rz_modmult' y x m size c A M;
+           CU (x,size - n) (mod_adder y size c (nat2fb ((2^m * A) mod M)) (nat2fb M))
    end.
 
 Definition rz_modmult_half y x size c A M := 
-   QFT y ;; rz_modmult' y x size size c A M ;; RQFT y.
+   QFT y ; rz_modmult' y x size size c A M ; RQFT y.
 
 Definition rz_modmult_full (y:var) (x:var) (n:nat) (c:posi) (A:nat) (Ainv :nat) (N:nat) :=
-  rz_modmult_half y x n c A N ;; inv_pexp (rz_modmult_half x y n c Ainv N).
+  rz_modmult_half y x n c A N ; inv_exp (rz_modmult_half x y n c Ainv N).
 
 Definition vars_for_rz' (size:nat) := gen_vars size (x_var::(y_var::[])).
 
@@ -100,271 +102,62 @@ Definition real_rz_modmult_rev (M C Cinv size:nat) :=
     rz_modmult_full y_var x_var size (z_var,0) C Cinv M.
 
 Definition trans_rz_modmult_rev (M C Cinv size:nat) :=
-        trans_pexp (vars_for_rz size) (2*size+1) (real_rz_modmult_rev M C Cinv size) (avs_for_arith size).
+        trans_exp (vars_for_rz size) (2*size+1) (real_rz_modmult_rev M C Cinv size) (avs_for_arith size).
 
 (*An alternative implementation for comparison on efficiency. *)
 Definition one_cu_sub (x:var) (n:nat) (c:posi) (M:nat -> bool) := CU c (rz_sub x n M).
 
 Definition rz_modadder_alt (c1:posi) (x:var) (n:nat) (c:posi) (A:nat -> bool) (M:nat -> bool) :=
-  Exp (one_cu_adder x n c1 A; (rz_sub x n M)) ;; qft_cu x c ;; Exp (one_cu_adder x n c M; one_cu_sub x n c1 A)
-      ;; qft_acu x c;; (Exp (one_cu_adder x n c1 A)).
+   (one_cu_adder x n c1 A; (rz_sub x n M)) ; qft_cu x c ;  (one_cu_adder x n c M; one_cu_sub x n c1 A)
+      ; qft_acu x c; ( (one_cu_adder x n c1 A)).
 
 Fixpoint rz_modmult_alt' (y:var) (x:var) (n:nat) (size:nat) (c:posi) (A:nat) (M:nat) :=
    match n with
-   | 0 => Exp (SKIP (y,0))
-   | S m => rz_modmult_alt' y x m size c A M;;
+   | 0 => (SKIP (y,0))
+   | S m => rz_modmult_alt' y x m size c A M;
             rz_modadder_alt (x,size-n) y size c (nat2fb ((2^m * A) mod M)) (nat2fb M)
    end.
 
 Definition rz_modmult_half_alt y x size c A M := 
-   QFT y ;; rz_modmult_alt' y x size size c A M ;; RQFT y.
+   QFT y ; rz_modmult_alt' y x size size c A M ; RQFT y.
 
 Definition rz_modmult_full_alt (y:var) (x:var) (n:nat) (c:posi) (A:nat) (Ainv :nat) (N:nat) :=
-  rz_modmult_half_alt y x n c A N ;; inv_pexp (rz_modmult_half_alt x y n c Ainv N).
+  rz_modmult_half_alt y x n c A N ; inv_exp (rz_modmult_half_alt x y n c Ainv N).
 
 Definition real_rz_modmult_rev_alt (M C Cinv size:nat) :=
     rz_modmult_full_alt y_var x_var size (z_var,0) C Cinv M.
 
 Definition trans_rz_modmult_rev_alt (M C Cinv size:nat) :=
-        trans_pexp (vars_for_rz size) (2*size+1) (real_rz_modmult_rev_alt M C Cinv size) (avs_for_arith size).
+        trans_exp (vars_for_rz size) (2*size+1) (real_rz_modmult_rev_alt M C Cinv size) (avs_for_arith size).
 
 
 (*********** Proofs ***********)
-
-Fixpoint natsum n (f : nat -> nat) :=
-  match n with
-  | 0 => 0
-  | S n' => f n' + natsum n' f
-  end.
-
-Lemma natsum_mod :
-  forall n f M,
-    M <> 0 ->
-    (natsum n f) mod M = natsum n (fun i => f i mod M) mod M.
+Lemma rz_adder_well_typed : forall n x size M aenv tenv, n <= size -> size = aenv x -> 
+           Env.MapsTo x (Phi (aenv x)) tenv -> well_typed_pexp aenv tenv (rz_adder' x n size M) tenv.
 Proof.
-  induction n; intros. easy.
-  simpl. rewrite Nat.add_mod by easy. rewrite IHn by easy. 
-  rewrite <- Nat.add_mod by easy. rewrite Nat.add_mod_idemp_l by easy. easy.
+ induction n; intros; simpl.
+ constructor. constructor.
+ apply pe_seq with (env' := tenv).
+ apply IHn; try easy. lia.
+ destruct (M n).
+ constructor.
+ apply sr_phi with (n := aenv x). easy.
+ subst. lia.
+ constructor. constructor.
 Qed.
 
-Lemma parity_decompose :
-  forall n, exists k, n = 2 * k \/ n = 2 * k + 1.
-Proof.
-  induction n. exists 0. lia. 
-  destruct IHn as [k [H | H]]. exists k. lia. exists (S k). lia.
-Qed.
-
-Lemma Natodd_Ntestbit_even :
-  forall k, Nat.odd (2 * k) = N.testbit (N.of_nat (2 * k)) 0.
-Proof.
-  induction k. easy.
-  replace (2 * (S k)) with (S (S (2 * k))) by lia.
-  rewrite Nat.odd_succ_succ. rewrite IHk.
-  do 2 rewrite N.bit0_odd.
-  replace (N.of_nat (S (S (2 * k)))) 
-   with (N.succ (N.succ (N.of_nat (2 * k)))) by lia.
-   rewrite N.odd_succ_succ. easy.
-Qed.
-
-Lemma Natodd_Ntestbit_odd :
-  forall k, Nat.odd (2 * k + 1) = N.testbit (N.of_nat (2 * k + 1)) 0.
-Proof.
-  induction k. easy.
-  replace (2 * (S k) + 1) with (S (S (2 * k + 1))) by lia.
-  rewrite Nat.odd_succ_succ. rewrite IHk.
-  do 2 rewrite N.bit0_odd.
-  replace (N.of_nat (S (S (2 * k + 1)))) 
-     with (N.succ (N.succ (N.of_nat (2 * k + 1)))) by lia.
-  rewrite N.odd_succ_succ. easy.
-Qed.
-
-Lemma nat_is_odd_testbit:
-  forall n, N.testbit (N.of_nat n) 0 = true -> Nat.odd n = true.
-Proof.
-  intros.
-  specialize (parity_decompose n) as [k [Hk | Hk]]; subst.
-  rewrite Natodd_Ntestbit_even.
-  assumption.
-  rewrite Natodd_Ntestbit_odd.
-  assumption.
-Qed.
-
-Lemma nat_is_even_testbit:
-  forall n, N.testbit (N.of_nat n) 0 = false -> Nat.even n = true.
-Proof.
-  intros.
-  assert (Nat.odd n = false).
-  specialize (parity_decompose n) as [k [Hk | Hk]]; subst.
-  rewrite Natodd_Ntestbit_even.
-  assumption.
-  rewrite Natodd_Ntestbit_odd.
-  assumption.
-  unfold Nat.odd in H0.
-  apply negb_false_iff in H0.
-  assumption.
-Qed.
-
-Lemma Nattestbit_Ntestbit :
-  forall m n,
-    Nat.testbit n m = N.testbit (N.of_nat n) (N.of_nat m).
-Proof.
-  induction m; intros. simpl. specialize (parity_decompose n) as [k [Hk | Hk]]; subst.
-   apply Natodd_Ntestbit_even. apply Natodd_Ntestbit_odd.
-  remember (N.of_nat (S m)) as NSm. simpl. rewrite IHm. rewrite Nnat.Nat2N.inj_div2.
-   rewrite <- N.testbit_succ_r_div2 by lia. subst. rewrite Nnat.Nat2N.inj_succ. easy.
-Qed.  
-
-Definition bindecomp n x := natsum n (fun i => Nat.b2n ((nat2fb x) i) * 2^i).
-
-Lemma bindecomp_spec :
-  forall n x,
-    bindecomp n x = x mod 2^n.
-Proof.
-  unfold bindecomp. induction n; intros. easy.
-  simpl. rewrite IHn. unfold nat2fb. rewrite N2fb_Ntestbit. rewrite <- Nattestbit_Ntestbit.
-  rewrite Nat.testbit_spec'. replace (2 ^ n + (2 ^ n + 0)) with ((2 ^ n) * 2) by lia. 
-  rewrite Nat.mod_mul_r. lia. apply Nat.pow_nonzero. easy. easy.
-Qed.
-
-Lemma bindecomp_seq :
-  forall n x, bindecomp (S n) x = bindecomp n x + Nat.b2n ((nat2fb x) n) * 2^n.
-Proof.
- intros.
- unfold bindecomp.
- simpl. lia.
-Qed.
-
-Lemma f_num_nat2fb : forall n f, (forall i, i >= n -> f i = false) -> (exists x, f = nat2fb x).
-Proof.
-  intros.
-  specialize (f_num_0 f n) as eq1.
-  destruct eq1.
-  assert (f = cut_n f n).
-  unfold cut_n.
-  apply functional_extensionality; intro.
-  bdestruct (x0 <? n). easy.
-  rewrite H. easy. easy.
-  exists x. rewrite H1. easy.
-Qed.
-
-Lemma add_to_sem : forall n q r, 0 < q <= n ->
-                 (forall i , i >= n -> r i = false) ->
-                 (addto r q) = cut_n (fbrev n (sumfb false (fbrev n r) (nat2fb (2^(n-q))))) n.
-Proof.
-  intros. unfold cut_n,addto,fbrev.
-  apply functional_extensionality; intro.
-  bdestruct (x <? q).
-  bdestruct (x <? n).
-Admitted. 
-
-Lemma add_to_n_sem : forall n q r, 0 < q <= n ->
-                 (forall i , i >= n -> r i = false) ->
-                 (addto_n r q) = cut_n (fbrev n (sumfb false (fbrev n r) (nat2fb (2^n - 2^(n-q))))) n.
-Proof.
-  intros. unfold addto_n.
-  apply functional_extensionality; intro.
-  bdestruct (x <? q).
-  rewrite negatem_arith.
-  assert ((forall i : nat, i >= n -> fbrev q r i = false)).
-  intros. unfold fbrev.
-  bdestruct (i <? q). lia. rewrite H0. easy. lia.
-  specialize (f_num_nat2fb n (fbrev q r) H2) as eq1.
-  destruct eq1.
-  rewrite H3.
-  rewrite cut_n_mod.
-  assert (2 ^ q <> 0).
-  apply Nat.pow_nonzero. lia.
-  rewrite sumfb_correct_carry0.
-  assert ((2 ^ q - 1 - 0) = ((2 ^ q -1) mod 2^q)).
-  rewrite Nat.mod_small by lia.
-  lia. rewrite H5.
-  rewrite cut_n_fbrev_flip.
-  rewrite cut_n_mod.
-  rewrite <- Nat.add_mod by lia.
-  assert (forall i : nat, i >= n -> fbrev n r i = false).
-  intros. unfold fbrev.
-  bdestruct (i <? n). lia. rewrite H0. easy. lia.
-  specialize (f_num_nat2fb n (fbrev n r) H6) as eq2.
-  destruct eq2.
-  rewrite H7.
-  rewrite sumfb_correct_carry0.
-  rewrite cut_n_fbrev_flip.
-  rewrite cut_n_mod.
-  Check Nat.add_mod.
-Admitted. 
-
-Lemma sumfb_assoc : forall f g h n, 
-          (forall i, i >= n -> f i = false) -> (forall i, i >= n -> g i = false) 
-             -> (forall i, i >= n -> h i = false) ->
-         sumfb false f (sumfb false g h) = sumfb false (sumfb false f g) h. 
-Proof.
-  intros.
-  rewrite <- (cut_n_eq n f).
-  rewrite <- (cut_n_eq n g).
-  rewrite <- (cut_n_eq n h).
-  specialize (f_num_0 f n) as eq1.
-  specialize (f_num_0 g n) as eq2.
-  specialize (f_num_0 h n) as eq3.
-  destruct eq1. destruct eq2. destruct eq3.
-  rewrite H2. rewrite H3. rewrite H4.
-  repeat rewrite sumfb_correct_carry0.
-  rewrite plus_assoc. easy.
-  easy. easy. easy.
-Qed.
-
-Definition get_phi_r (v:val) := match v with qval r1 r2 => r2 | _ => allfalse end.
-
-Lemma sr_rotate_get_r : forall n size f x, 0 < n <= size -> get_r_qft (sr_rotate' f x n size) x
-                 = get_phi_r (times_rotate (f (x,0)) size).
-Proof.
-  induction n;intros; simpl. lia.
-  unfold get_r_qft.
-  bdestruct (n =? 0). subst. 
-  rewrite eupdate_index_eq.
-  unfold get_phi_r.
-  assert (size - 0=size) by lia. rewrite H0. easy.
-  rewrite eupdate_index_neq by iner_p.
-  unfold get_r_qft in IHn. rewrite IHn. easy. lia.
-Qed.
-
-Lemma sr_rotate'_phi : forall m n size f x, m <= n <= size -> phi_modes f x size
-             -> phi_modes ((sr_rotate' f x m n)) x size.
-Proof.
-  induction m; intros ; simpl; try easy.
-  unfold phi_modes in *. intros.
-  unfold phi_mode in *. 
-  bdestruct (m =? i). subst.
-  rewrite eupdate_index_eq.
-  unfold times_rotate.
-  apply H0 in H1. destruct (f (x,i)) eqn:eq1. lia. lia. lia.
-  rewrite eupdate_index_neq by iner_p.
-  apply IHm with (size := size). lia. easy. lia.
-Qed.
-
-Lemma rz_adder_well_typed : forall n x size M f aenv tenv, n <= size ->
-             phi_modes f x size -> well_typed_exp tenv (rz_adder' x n size M)
-             -> right_mode_env aenv tenv f -> phi_modes (exp_sem aenv (rz_adder' x n size M) f) x size.
+Lemma rz_adder_phi_modes : forall n x size M f aenv tenv, n <= size -> size = aenv x ->
+           Env.MapsTo x (Phi (aenv x)) tenv -> right_mode_env aenv tenv f -> 
+             phi_modes (exp_sem aenv (rz_adder' x n size M) f) x size.
 Proof.
   induction n; intros.
-  simpl in *. easy.
-  simpl in *.
-  inv H1.
-  specialize (IHn x size M f aenv tenv).
-  assert (n <= size) by lia.
-  specialize (IHn H1 H0 H6 H2).
-  unfold phi_modes in *. 
-  intros.
-  unfold phi_mode in *.
-  destruct (M n) eqn:eq1. simpl.
-  unfold sr_rotate.
-  specialize (sr_rotate'_phi (S (size - S n)) (S (size - S n)) size 
-                 (exp_sem aenv (rz_adder' x n size M) f) x) as eq2.
-  assert (S (size - S n) <= S (size - S n) <= size) by lia.
-  assert (phi_modes (exp_sem aenv (rz_adder' x n size M) f) x size).
-  unfold phi_modes. unfold phi_mode. apply IHn.
-  specialize (eq2 H4 H5).
-  unfold phi_modes in eq2. unfold phi_mode in eq2. apply eq2; try lia.
-  simpl. apply IHn; lia.
+  simpl in *. rewrite H0. apply type_phi_modes with (env := tenv); easy.
+  simpl.
+  destruct (M n).
+  apply sr_phi_modes.
+  apply IHn with (tenv := tenv); try easy. lia.
+  simpl.
+  apply IHn with (tenv := tenv); try easy. lia.
 Qed. 
 
 Lemma rz_adder_gt : forall n size aenv M f x, n <= size ->
@@ -397,9 +190,8 @@ Proof.
   simpl. apply IHn. lia. apply H0. lia.
 Qed.
 
-Lemma rz_adder_sem : forall n size f x A M aenv tenv, n <= size -> phi_modes f x size ->
-                 (forall i, i <= size -> well_typed_exp tenv (rz_adder' x i size (nat2fb M)))
-                   -> right_mode_env aenv tenv f ->
+Lemma rz_adder_sem : forall n size f x A M aenv tenv, n <= size -> size = aenv x ->
+                  Env.MapsTo x (Phi (aenv x)) tenv -> right_mode_env aenv tenv f ->
                   M < 2^size -> A < 2^size ->
                   fbrev size (get_r_qft f x) = nat2fb A ->
                   (get_r_qft (exp_sem aenv (rz_adder' x n size (nat2fb M)) f) x)
@@ -420,13 +212,12 @@ Proof.
   assert (n <= size) by lia.
   specialize (IHn H6 H0 H1 H2 H3 H4 H5).
   unfold get_r_qft in IHn.
-  specialize (H1 n H6).
-  apply rz_adder_well_typed with (aenv:=aenv) (f:= f) in H1 as eq3; try easy.
+  specialize (rz_adder_phi_modes n x size (nat2fb M) f aenv tenv H6 H0 H1 H2) as eq3.
   unfold phi_modes in eq3. assert (0 < size) by lia. specialize (eq3 0 H7).
   unfold phi_mode in eq3.
   specialize (rz_adder_gt n size aenv (nat2fb M) f x) as X1.
   assert (n <= size) by lia.
-  specialize (X1 H6).
+  specialize (X1 H8).
   assert ((forall i : nat, i >= size -> get_r_qft f x i = false)).
   intros.
   specialize (nat2fb_bound size A H4 i H9) as X2.
@@ -434,7 +225,8 @@ Proof.
   unfold fbrev in X2. bdestruct (i <? size). lia.
   easy. specialize (X1 H9).
   unfold get_r_qft in X1.
-  destruct (exp_sem aenv (rz_adder' x n size (nat2fb M)) f (x, 0)) eqn:eq2. lia. lia.
+  destruct (exp_sem aenv (rz_adder' x n size (nat2fb M)) f (@pair var nat x O)) eqn:eq2.
+   lia. lia.
   unfold times_rotate,rotate.
   rewrite (add_to_sem size); (try easy; try lia).
   rewrite cut_n_fbrev_flip.
@@ -457,6 +249,21 @@ Proof.
   rewrite IHn with (A := A) (tenv:=tenv); try easy.
   rewrite bindecomp_seq.
   rewrite eq1. simpl. rewrite plus_0_r. easy. lia.
+Qed.
+
+(*
+Lemma rz_adder_well_typed : forall n x size M aenv tenv, n <= size -> size = aenv x -> 
+           Env.MapsTo x (Phi (aenv x)) tenv -> well_typed_pexp aenv tenv (rz_adder' x n size M) tenv.
+Proof.
+ induction n; intros; simpl.
+ constructor. constructor.
+ apply pe_seq with (env' := tenv).
+ apply IHn; try easy. lia.
+ destruct (M n).
+ constructor.
+ apply sr_phi with (n := aenv x). easy.
+ subst. lia.
+ constructor. constructor.
 Qed.
 
 Lemma well_typed_exp_rz_adder_aux : forall m size tenv f x M, S m <= size 
@@ -499,10 +306,10 @@ Proof.
  rewrite H2 in H0.
  apply well_typed_exp_rz_adder_1 with (f:=f) in H0. easy. lia. easy.
 Qed.
+*)
 
-Lemma rz_adder_full : forall size f x A M aenv tenv, phi_modes f x size ->
-                   well_typed_exp tenv (rz_adder x size (nat2fb M))
-                   -> right_mode_env aenv tenv f ->
+Lemma rz_adder_full : forall size f x A M aenv tenv, size = aenv x ->
+                  Env.MapsTo x (Phi (aenv x)) tenv -> right_mode_env aenv tenv f ->
                   M < 2^size -> A < 2^size ->
                   fbrev size (get_r_qft f x) = nat2fb A ->
                   (get_r_qft (exp_sem aenv (rz_adder x size (nat2fb M)) f) x)
@@ -511,60 +318,34 @@ Proof.
   intros. unfold rz_adder. rewrite rz_adder_sem with (A:=A) (tenv := tenv); try easy.
   rewrite bindecomp_spec.
   rewrite (Nat.mod_small M) by easy. easy.
-  apply well_typed_exp_rz_adder with (f:=f); easy.
 Qed.
 
-Lemma srr_rotate_get_r : forall n size f x, 0 < n <= size -> get_r_qft (srr_rotate' f x n size) x
-                 = get_phi_r (times_r_rotate (f (x,0)) size).
+Lemma rz_sub_well_typed : forall n x size M aenv tenv, n <= size -> size = aenv x -> 
+           Env.MapsTo x (Phi (aenv x)) tenv -> well_typed_pexp aenv tenv (rz_sub' x n size M) tenv.
 Proof.
-  induction n;intros; simpl. lia.
-  unfold get_r_qft.
-  bdestruct (n =? 0). subst. 
-  rewrite eupdate_index_eq.
-  unfold get_phi_r.
-  assert (size - 0=size) by lia. rewrite H0. easy.
-  rewrite eupdate_index_neq by iner_p.
-  unfold get_r_qft in IHn. rewrite IHn. easy. lia.
+ induction n; intros; simpl.
+ constructor. constructor.
+ apply pe_seq with (env' := tenv).
+ apply IHn; try easy. lia.
+ destruct (M n).
+ constructor.
+ apply srr_phi with (n := aenv x). easy.
+ subst. lia.
+ constructor. constructor.
 Qed.
 
-Lemma srr_rotate'_phi : forall m n size f x, m <= n <= size -> phi_modes f x size
-             -> phi_modes ((srr_rotate' f x m n)) x size.
-Proof.
-  induction m; intros ; simpl; try easy.
-  unfold phi_modes in *. intros.
-  unfold phi_mode in *. 
-  bdestruct (m =? i). subst.
-  rewrite eupdate_index_eq.
-  unfold times_r_rotate.
-  apply H0 in H1. destruct (f (x,i)) eqn:eq1. lia. lia. lia.
-  rewrite eupdate_index_neq by iner_p.
-  apply IHm with (size := size). lia. easy. lia.
-Qed.
-
-Lemma rz_sub_well_typed : forall n x size M f aenv tenv, n <= size ->
-             phi_modes f x size -> well_typed_exp tenv (rz_sub' x n size M)
-             -> right_mode_env aenv tenv f -> phi_modes (exp_sem aenv (rz_sub' x n size M) f) x size.
+Lemma rz_sub_phi_modes : forall n x size M f aenv tenv, n <= size -> size = aenv x ->
+           Env.MapsTo x (Phi (aenv x)) tenv -> right_mode_env aenv tenv f -> 
+             phi_modes (exp_sem aenv (rz_sub' x n size M) f) x size.
 Proof.
   induction n; intros.
-  simpl in *. easy.
-  simpl in *.
-  inv H1.
-  specialize (IHn x size M f aenv tenv).
-  assert (n <= size) by lia.
-  specialize (IHn H1 H0 H6 H2).
-  unfold phi_modes in *. 
-  intros.
-  unfold phi_mode in *.
-  destruct (M n) eqn:eq1. simpl.
-  unfold srr_rotate.
-  specialize (srr_rotate'_phi (S (size - S n)) (S (size - S n)) size 
-                 (exp_sem aenv (rz_sub' x n size M) f) x) as eq2.
-  assert (S (size - S n) <= S (size - S n) <= size) by lia.
-  assert (phi_modes (exp_sem aenv (rz_sub' x n size M) f) x size).
-  unfold phi_modes. unfold phi_mode. apply IHn.
-  specialize (eq2 H4 H5).
-  unfold phi_modes in eq2. unfold phi_mode in eq2. apply eq2; try lia.
-  simpl. apply IHn; lia.
+  simpl in *. rewrite H0. apply type_phi_modes with (env := tenv); easy.
+  simpl.
+  destruct (M n).
+  apply srr_phi_modes.
+  apply IHn with (tenv := tenv); try easy. lia.
+  simpl.
+  apply IHn with (tenv := tenv); try easy. lia.
 Qed. 
 
 Lemma rz_sub_gt : forall n size aenv M f x, n <= size ->
@@ -597,9 +378,8 @@ Proof.
   simpl. apply IHn. lia. apply H0. lia.
 Qed.
 
-Lemma rz_sub_sem : forall n size f x A M aenv tenv, n <= size -> phi_modes f x size ->
-                 (forall i, i <= size -> well_typed_exp tenv (rz_sub' x i size (nat2fb M)))
-                   -> right_mode_env aenv tenv f ->
+Lemma rz_sub_sem : forall n size f x A M aenv tenv, n <= size -> size = aenv x ->
+                  Env.MapsTo x (Phi (aenv x)) tenv -> right_mode_env aenv tenv f ->
                   M < 2^size -> A < 2^size ->
                   fbrev size (get_r_qft f x) = nat2fb A ->
                   (get_r_qft (exp_sem aenv (rz_sub' x n size (nat2fb M)) f) x)
@@ -624,13 +404,12 @@ Proof.
   assert (n <= size) by lia.
   specialize (IHn H6 H0 H1 H2 H3 H4 H5).
   unfold get_r_qft in IHn.
-  specialize (H1 n H6).
-  apply rz_sub_well_typed with (aenv:=aenv) (f:= f) in H1 as eq3; try easy.
+  specialize (rz_sub_phi_modes n x size (nat2fb M) f aenv tenv H6 H0 H1 H2) as eq3.
   unfold phi_modes in eq3. assert (0 < size) by lia. specialize (eq3 0 H7).
   unfold phi_mode in eq3.
   specialize (rz_sub_gt n size aenv (nat2fb M) f x) as X1.
   assert (n <= size) by lia.
-  specialize (X1 H6).
+  specialize (X1 H8).
   assert ((forall i : nat, i >= size -> get_r_qft f x i = false)).
   intros.
   specialize (nat2fb_bound size A H4 i H9) as X2.
@@ -638,7 +417,7 @@ Proof.
   unfold fbrev in X2. bdestruct (i <? size). lia.
   easy. specialize (X1 H9).
   unfold get_r_qft in X1.
-  destruct (exp_sem aenv (rz_sub' x n size (nat2fb M)) f (x, 0)) eqn:eq2. lia. lia.
+  destruct (exp_sem aenv (rz_sub' x n size (nat2fb M)) f (@pair var nat x O)) eqn:eq2. lia. lia.
   unfold times_r_rotate,r_rotate.
   rewrite (add_to_n_sem size); (try easy; try lia).
   rewrite cut_n_fbrev_flip.
@@ -675,7 +454,7 @@ Proof.
   rewrite eq1. simpl. rewrite plus_0_r. easy. lia.
 Qed.
 
-
+(*
 Lemma well_typed_exp_rz_sub_aux : forall m size tenv f x M, S m <= size 
             -> phi_modes f x size
            -> well_typed_exp tenv (rz_sub' x (S m) size (nat2fb M))
@@ -716,10 +495,10 @@ Proof.
  rewrite H2 in H0.
  apply well_typed_exp_rz_sub_1 with (f:=f) in H0. easy. lia. easy.
 Qed.
+*)
 
-Lemma rz_sub_full : forall size f x A M aenv tenv, phi_modes f x size ->
-                    well_typed_exp tenv (rz_sub x size (nat2fb M))
-                   -> right_mode_env aenv tenv f ->
+Lemma rz_sub_full : forall size f x A M aenv tenv, size = aenv x ->
+                  Env.MapsTo x (Phi (aenv x)) tenv -> right_mode_env aenv tenv f ->
                   M < 2^size -> A < 2^size ->
                   fbrev size (get_r_qft f x) = nat2fb A ->
                   (get_r_qft (exp_sem aenv (rz_sub x size (nat2fb M)) f) x)
@@ -728,7 +507,6 @@ Proof.
   intros. unfold rz_sub. rewrite rz_sub_sem with (A:=A) (tenv := tenv); try easy.
   rewrite bindecomp_spec.
   rewrite (Nat.mod_small M) by easy. easy.
-  apply well_typed_exp_rz_sub with (f := f); easy.
 Qed.
 
 Lemma efresh_rz_adder: forall n c x size M aenv, fst c <> x -> n <= size -> exp_fresh aenv c (rz_adder' x n size M).
@@ -753,71 +531,60 @@ Proof.
   constructor. destruct c. iner_p.
 Qed.
 
-Lemma highbit_means_lt : forall size X M, X < 2^ S size -> M < 2^size -> X < 2 * M 
-         -> fbrev (S size) (nat2fb ((X + 2^S size - M) mod 2^S size)) 0 = (X <? M).
+Lemma rz_compare_half_well_typed : forall x c size M aenv tenv, 
+           x <> fst c -> size = aenv x -> 
+           Env.MapsTo (fst c) Nor tenv -> Env.MapsTo x (Phi (aenv x)) tenv ->
+           well_typed_pexp aenv tenv (rz_compare_half x size c M) (Env.add x Nor tenv).
 Proof.
-  intros. unfold fbrev.
-  bdestruct (0 <? size). simpl.
-  assert ((size - 0 - 0) = size) by lia. rewrite H3.
-  unfold nat2fb.
-  rewrite N2fb_Ntestbit.
-  bdestruct (X <? M).
-  apply Ntestbit_in_pow2n_pow2Sn.
-  assert ((2 ^ size + (2 ^ size + 0)) = 2^ S size). simpl. easy.
-  rewrite H5.
-  split.
-  assert (2^size <= (X + 2 ^ S size - M) mod 2 ^ S size).
-  assert ((X + 2 ^ S size - M) = 2^S size - (M - X)) by lia.
-  rewrite H6.
-  assert ((2 ^ S size - (M - X)) < 2 ^ S size) by lia.
-  rewrite Nat.mod_small by lia.
-  assert (M - X < 2^size) by lia. lia.
-  assert (N.of_nat(2 ^ size) <= N.of_nat ((X + 2 ^ S size - M) mod 2 ^ S size))%N by lia.
-  simpl in *. rewrite Nofnat_pow in H7. simpl in H7. lia.
-  assert ((X + 2 ^ S size - M) mod 2 ^ S size < 2 ^ S size).
-  apply Nat.mod_upper_bound. lia.
-  assert (N.of_nat ((X + 2 ^ S size - M) mod 2 ^ S size) < N.of_nat (2 ^ S size))%N by lia.
-  rewrite Nofnat_pow in H7. 
-  assert (N.of_nat (S size) = N.succ (N.of_nat size)) by lia.
-  rewrite H8 in H7. simpl in *. lia.
-  apply Ntestbit_lt_pow2n.
-  assert ((2 ^ size + (2 ^ size + 0)) = 2^ S size). simpl. easy.
-  rewrite H5. clear H5.
-  assert ((X + 2 ^ S size - M) mod 2 ^ S size < 2 ^ size).
-  assert ((X + 2 ^ S size - M) = 2 ^ S size + (X - M)) by lia.
-  rewrite H5. clear H5.
-  assert (2^ size <> 0).
-  apply Nat.pow_nonzero. lia.
-  rewrite Nat.add_mod by (simpl;lia).
-  rewrite Nat.mod_same by (simpl;lia).
-  rewrite plus_0_l.
-  rewrite Nat.mod_mod by (simpl;lia).
-  rewrite Nat.mod_small by (simpl;lia).
-  simpl. lia.
-  assert (N.of_nat ((X + 2 ^ S size - M) mod 2 ^ S size) < N.of_nat (2 ^ size))%N by lia.
-  rewrite Nofnat_pow in H6. 
-  simpl in *. lia. 
-  bdestruct (0 <? S size).
-  assert (size = 0) by lia. subst. simpl in *. lia.
-  lia.
+ intros. unfold rz_compare_half.
+ apply pe_seq with (env' := (Env.add x Nor tenv)).
+ apply pe_seq with (env' := tenv).
+ apply rz_sub_well_typed; try easy.
+ apply rqft_phi. easy. easy.
+ apply cnot_wt_nor. iner_p.
+ simpl. apply Env.add_1. easy.
+ simpl. apply Env.add_2. easy. easy.
 Qed.
 
-Lemma rz_compare_half_sem : forall size f c x A M aenv l l' tenv tenv',
-                    phi_modes f x (S size) -> aenv x = S size -> fst c <> x
-                     -> nor_mode f c -> get_cua (f c) = false ->
-                    well_typed_pexp aenv l tenv (rz_compare_half x (S size) c M) l' tenv'
-                   -> right_mode_env aenv tenv f ->
-                  M < 2^size -> A < 2^S size -> A < 2*M ->
-                  fbrev (S size) (get_r_qft f x) = nat2fb A ->
-                  get_cua ((prog_sem aenv (rz_compare_half x (S size) c M) f) c) = (A <? M).
+(*
+Lemma rz_compare_half_phi_modes : forall x c size M f aenv tenv,
+           x <> fst c -> size = aenv x -> 
+           Env.MapsTo (fst c) Nor tenv -> Env.MapsTo x (Phi (aenv x)) tenv ->
+           right_mode_env aenv tenv f -> 
+             nor_modes (exp_sem aenv (rz_compare_half x size c M) f) x size.
 Proof.
-  intros. unfold rz_compare_half. 
+ intros. unfold rz_compare_half.
+ assert ((exp_sem aenv ((rz_sub x size (nat2fb M); RQFT x); CNOT (@pair var nat x O) c) f)
+   = exp_sem aenv (CNOT (@pair var nat x O) c) (exp_sem aenv (RQFT x) (exp_sem aenv (rz_sub x size (nat2fb M)) f))).
+ simpl. easy.
+ rewrite H4. clear H4.
+Admitted. 
+*)
+
+Lemma rz_compare_half_sem : forall size f c x A M aenv tenv,
+            aenv x = S size -> fst c <> x -> Env.MapsTo x (Phi (aenv x)) tenv -> 
+            Env.MapsTo (fst c) Nor tenv -> get_cua (f c) = false ->
+            right_mode_env aenv tenv f -> snd c < aenv (fst c)
+            -> M < 2^size -> A < 2^S size -> A < 2*M ->
+            fbrev (S size) (get_r_qft f x) = nat2fb A ->
+                  get_cua ((exp_sem aenv (rz_compare_half x (S size) c M) f) c) = (A <? M).
+Proof.
+  intros. unfold rz_compare_half.
+  assert (well_typed_pexp aenv tenv (rz_sub x (S size) (nat2fb M)) tenv) as X1.
+  apply rz_sub_well_typed; try easy.
+  assert (well_typed_pexp aenv tenv (RQFT x) (Env.add x Nor tenv)) as X2.
+  apply rqft_phi; try easy.
+  assert (well_typed_pexp aenv (Env.add x Nor tenv) (CNOT (@pair var nat x O) c) (Env.add x Nor tenv)) as X3.
+  apply cnot_wt_nor. destruct c. iner_p.
+  simpl. apply Env.add_1. easy.
+  apply Env.add_2. iner_p. easy.
+  assert (nor_mode f c) as X4.
+  apply type_nor_mode with (aenv := aenv) (env := tenv); try easy.
   remember (rz_sub x (S size) (nat2fb M)) as e1. simpl.
-  rewrite Heqe1. clear Heqe1.
+  rewrite Heqe1 in *. clear Heqe1.
   unfold turn_rqft.
-  inv H4. inv H14. inv H13.
-  rewrite rz_sub_full with (A:=A) (tenv:= env'0); try easy.
-  rewrite H0.
+  rewrite rz_sub_full with (A:=A) (tenv:= tenv); try easy.
+  unfold rz_compare_half in X1. 
   rewrite cnot_sem.
   rewrite eupdate_index_eq.
   rewrite get_put_cu.
@@ -827,53 +594,57 @@ Proof.
   rewrite H3.
   unfold get_cua. bt_simpl.
   unfold fbrev. bdestruct (0 <? S size). simpl.
-  assert ((size - 0 - 0) = size) by lia. rewrite H12.
+  assert ((size - 0 - 0) = size) by lia. rewrite H11.
   rewrite <- highbit_means_lt with (size := size); try easy.
   unfold fbrev.
   bdestruct (0 <? S size). simpl.
-  rewrite H12. easy. lia. lia.
+  rewrite H11. easy. lia. lia.
   apply efresh_rz_sub; try easy.
   unfold nor_mode.
   rewrite assign_seq_out by iner_p.
   rewrite efresh_exp_sem_irrelevant with (p := c).
-  apply H2.
+  apply X4.
   apply efresh_rz_sub; try easy.
   unfold nor_mode.
   rewrite assign_seq_lt by lia. lia.
   unfold nor_mode.
   rewrite assign_seq_out by iner_p.
   rewrite efresh_exp_sem_irrelevant with (p := c).
-  apply H2.
+  apply X4.
   apply efresh_rz_sub; try easy.
   simpl. lia.
 Qed.
 
-Lemma rz_compare_sem : forall size f c x A M aenv l l' tenv tenv',
-                    phi_modes f x (S size) -> aenv x = S size -> fst c <> x
-                     -> nor_mode f c -> get_cua (f c) = false ->
-                    well_typed_pexp aenv l tenv (rz_compare_half x (S size) c M) l' tenv'
-                   -> right_mode_env aenv tenv f -> qft_uniform aenv tenv f -> qft_gt aenv tenv f ->
-                  pexp_fresh aenv c (Exp (rz_sub x (S size) (nat2fb M));; RQFT x) ->
-                  M < 2^size -> A < 2^size ->
-                  fbrev (S size) (get_r_qft f x) = nat2fb A ->
-                  well_formed_ls l -> exp_neu_prop l ->
-                     prog_sem aenv (rz_compare x (S size) c M) f = f[c|-> put_cu (f c) (A <? M)].
+Lemma rz_compare_sem : forall size f c x A M aenv tenv,
+            aenv x = S size -> fst c <> x -> Env.MapsTo x (Phi (aenv x)) tenv -> 
+            Env.MapsTo (fst c) Nor tenv -> get_cua (f c) = false -> snd c < aenv (fst c)
+            -> M < 2^size -> A < 2^S size -> A < 2*M -> get_cua (f c) = false 
+            -> right_mode_env aenv tenv f -> qft_uniform aenv tenv f -> qft_gt aenv tenv f ->
+               M < 2^size -> A < 2^size -> fbrev (S size) (get_r_qft f x) = nat2fb A ->
+                     exp_sem aenv (rz_compare x (S size) c M) f = f[c|-> put_cu (f c) (A <? M)].
 Proof.
   intros. unfold rz_compare. unfold rz_compare_half in *. 
-  inv H4.
-  remember (rz_sub x (S size) (nat2fb M);; RQFT x) as e1. 
-  remember (prog_sem aenv e1 f) as g.
+  assert (well_typed_pexp aenv tenv (rz_sub x (S size) (nat2fb M)) tenv) as X1.
+  apply rz_sub_well_typed; try easy.
+  assert (well_typed_pexp aenv tenv (RQFT x) (Env.add x Nor tenv)) as X2.
+  apply rqft_phi; try easy.
+  assert (well_typed_pexp aenv (Env.add x Nor tenv) (CNOT (@pair var nat x O) c) (Env.add x Nor tenv)) as X3.
+  apply cnot_wt_nor. destruct c. iner_p.
+  simpl. apply Env.add_1. easy.
+  apply Env.add_2. iner_p. easy.
+  assert (nor_mode f c) as X4.
+  apply type_nor_mode with (aenv := aenv) (env := tenv); try easy.
+  remember (rz_sub x (S size) (nat2fb M); RQFT x) as e1. 
+  remember (exp_sem aenv e1 f) as g.
   simpl.
   rewrite <- Heqg.
   rewrite cnot_sem.
-  rewrite inv_pexp_reverse_1 with (tenv:= tenv) (tenv' := env') (f:=f) (l := l) (l' := l'0); try easy.
+  rewrite inv_pexp_reverse_1 with (tenv:= tenv) (tenv' := (Env.add x Nor tenv)) (f:=f); try easy.
   rewrite Heqg.
   rewrite Heqe1 in *.
   remember (rz_sub x (S size) (nat2fb M)) as e2. simpl in *.
-  unfold turn_rqft.
-  inv H18. inv H17.
-  rewrite rz_sub_full with (A:=A) (tenv:= env'0); try easy.
-  rewrite H0.
+  unfold turn_rqft. rewrite Heqe2 in *.
+  rewrite rz_sub_full with (A:=A) (tenv:= tenv); try easy.
   rewrite assign_seq_lt by lia.
   rewrite assign_seq_out by iner_p.
   rewrite efresh_exp_sem_irrelevant with (p := c).
@@ -892,18 +663,18 @@ Proof.
   split.
   assert (2^size <= (A + 2 ^ S size - M) mod 2 ^ S size).
   assert ((A + 2 ^ S size - M) = 2^S size - (M - A)) by lia.
-  rewrite H20.
+  rewrite H19.
   assert ((2 ^ S size - (M - A)) < 2 ^ S size) by lia.
   rewrite Nat.mod_small by lia.
   assert (M - A < 2^size) by lia. lia.
   assert (N.of_nat(2 ^ size) <= N.of_nat ((A + 2 ^ S size - M) mod 2 ^ S size))%N by lia.
-  simpl in *. rewrite Nofnat_pow in H23. simpl in H23. lia.
+  simpl in *. rewrite Nofnat_pow in H20. simpl in H20. lia.
   assert ((A + 2 ^ S size - M) mod 2 ^ S size < 2 ^ S size).
   apply Nat.mod_upper_bound. lia.
   assert (N.of_nat ((A + 2 ^ S size - M) mod 2 ^ S size) < N.of_nat (2 ^ S size))%N by lia.
-  rewrite Nofnat_pow in H23. 
+  rewrite Nofnat_pow in H20. 
   assert (N.of_nat (S size) = N.succ (N.of_nat size)) by lia.
-  rewrite H24 in H23. simpl in *. lia.
+  rewrite H21 in H20. simpl in *. lia.
   apply Ntestbit_lt_pow2n.
   assert ((2 ^ size + (2 ^ size + 0)) = 2^ S size). simpl. easy.
   rewrite H18. clear H18.
@@ -919,16 +690,26 @@ Proof.
   rewrite Nat.mod_small by (simpl;lia).
   simpl. lia.
   assert (N.of_nat ((A + 2 ^ S size - M) mod 2 ^ S size) < N.of_nat (2 ^ size))%N by lia.
-  rewrite Nofnat_pow in H20. 
+  rewrite Nofnat_pow in H19. 
   simpl in *. lia. rewrite H17. easy. lia.
-  inv H8. inv H18. easy. simpl. lia. simpl. lia.
+  apply efresh_rz_sub; try easy. simpl. lia.
+  subst. 
+  apply pe_seq with (env' := tenv).
+  easy. easy.
+  subst. 
+  constructor. 
+  apply efresh_rz_sub; try easy.
+  constructor. unfold or_not_eq. left. easy.
   subst. simpl. unfold turn_rqft.
   unfold nor_mode. simpl.
-  rewrite assign_seq_lt. lia. rewrite H0. lia.
-  subst.
+  rewrite assign_seq_lt. lia. rewrite H. lia.
+  subst. 
   unfold nor_mode.
-  rewrite fresh_pexp_sem_irrelevant with (p := c).
-  apply H2. easy.
+  rewrite efresh_exp_sem_irrelevant with (p := c).
+  apply X4.
+  constructor. 
+  apply efresh_rz_sub; try easy.
+  constructor. unfold or_not_eq. left. easy.
 Qed.
 
 
@@ -1118,23 +899,21 @@ Proof.
   apply H0. inv H. lia. lia.
   simpl. apply H0. lia. simpl. apply H0. lia.
   simpl.
+  inv H. inv H. inv H.
   inv H.
   specialize (IHe1 aenv f x size H5 H0).
   specialize (IHe2 aenv (exp_sem aenv e1 f) x size H6 IHe1). easy.
 Qed.
 
 Lemma adder_sub_seq : forall size f x B A M aenv tenv,
-                 phi_modes f x size -> exp_scope aenv x size (rz_adder x size (nat2fb A))
-                 ->  well_typed_exp tenv (rz_adder x size (nat2fb A))
-                -> well_typed_exp tenv (rz_sub x size (nat2fb M))
-                   -> right_mode_env aenv tenv f -> 
+            size = aenv x -> Env.MapsTo x (Phi (aenv x)) tenv -> right_mode_env aenv tenv f -> 
                   1 < M < 2^size -> A < 2^size -> B < 2^size ->
                   fbrev size (get_r_qft f x) = nat2fb B ->
                   (get_r_qft (exp_sem aenv (rz_adder x size (nat2fb A); (rz_sub x size (nat2fb M))) f) x)
                     = (fbrev size (nat2fb (((B + A) + 2^size - M) mod 2^size))).
 Proof.
   intros.
-  specialize (rz_adder_full size f x B A aenv tenv H H1 H3 H5 H6 H7) as eq1.
+  specialize (rz_adder_full size f x B A aenv tenv H H0 H1 H3 H4 H5) as eq1.
   simpl.
   assert (fbrev size (get_r_qft (exp_sem aenv (rz_adder x size (nat2fb A)) f) x) 
                = (nat2fb ((B + A) mod 2 ^ size))).
@@ -1144,64 +923,67 @@ Proof.
   rewrite Nat.mod_small by lia. easy.
   assert (((B + A) mod 2 ^ size + 2 ^ size - M) =
               ((B + A) mod 2 ^ size + (2 ^ size - M))) by lia.
-  rewrite H10. rewrite H9.
+  rewrite H8. rewrite H7.
   rewrite <- Nat.add_mod by lia.
   assert ((B + A + (2 ^ size - M)) = ((B + A + 2 ^ size - M))) by lia.
-  rewrite H11. easy.
-  apply phi_modes_exp. easy. easy.
-  apply well_typed_right_mode_exp; try easy.
+  rewrite H9. easy.
+  apply well_typed_right_mode_pexp with (tenv := tenv); try easy.
+  apply rz_adder_well_typed; try easy.
   apply Nat.mod_upper_bound. lia.
 Qed.
 
-Lemma qft_cu_sem : forall l tenv tenv' aenv f x c size, phi_modes f x (S size) -> aenv x = S size
-          -> nor_mode f c -> fst c <> x ->
-          well_typed_pexp aenv l tenv (RQFT x) l tenv' -> right_mode_env aenv tenv f ->
-           qft_uniform aenv tenv f -> qft_gt aenv tenv f ->
-                  well_formed_ls l -> exp_neu_prop l ->
-          prog_sem aenv (qft_cu x c) f = f[c |-> put_cu (f c) ((get_r_qft f x 0) ⊕ get_cua (f c))].
+Lemma qft_cu_sem : forall tenv aenv f x c size,
+            aenv x = S size -> fst c <> x -> Env.MapsTo x (Phi (aenv x)) tenv -> 
+            Env.MapsTo (fst c) Nor tenv -> snd c < aenv (fst c) ->
+             right_mode_env aenv tenv f -> qft_uniform aenv tenv f -> qft_gt aenv tenv f ->
+          exp_sem aenv (qft_cu x c) f = f[c |-> put_cu (f c) ((get_r_qft f x 0) ⊕ get_cua (f c))].
 Proof.
   intros.
   unfold qft_cu.
   remember (RQFT x) as e.
-  assert (QFT x = inv_pexp e). rewrite Heqe. simpl. easy.
-  rewrite H9. simpl.
+  assert (QFT x = inv_exp e). rewrite Heqe. simpl. easy.
+  rewrite H7. simpl.
   rewrite cnot_sem.
-  rewrite fresh_pexp_sem_out.
-  assert ((prog_sem aenv (inv_pexp e) (prog_sem aenv e f))
-          = prog_sem aenv (e ;; inv_pexp e) f). simpl. easy.
-  rewrite H10.
-  rewrite inv_pexp_correct_rev with (tenv := tenv) (tenv' := tenv') (l:= l) (l':=l); try easy.
+  rewrite efresh_exp_sem_out.
+  assert ((exp_sem aenv (inv_exp e) (exp_sem aenv e f))
+          = exp_sem aenv (e ; inv_exp e) f). simpl. easy.
+  rewrite H8.
+  rewrite inv_exp_correct_rev with (tenv := tenv) (tenv' := Env.add x Nor tenv); try easy.
   apply eupdate_same_1. easy.
   rewrite Heqe. simpl.
   unfold turn_rqft,turn_qft.
   rewrite assign_seq_out; try iner_p.
   rewrite assign_seq_lt; try lia.
-  assert (get_cua (nval (get_r_qft f x 0) (get_r (f (x, 0)))) = (get_r_qft f x 0)).
+  assert (get_cua (nval (get_r_qft f x 0) (get_r (f (@pair var nat x O)))) = (get_r_qft f x 0)).
   unfold get_cua. easy.
-  rewrite H11. easy.
-  rewrite Heqe. simpl. constructor.
-  unfold or_not_eq. left. lia.
+  rewrite H9. easy.
+  rewrite Heqe.
+  apply rqft_phi. easy.
+  easy.
+  rewrite Heqe. simpl.
+  constructor. unfold or_not_eq. left. easy.
   rewrite Heqe. simpl.
   unfold turn_rqft.
   unfold nor_mode.
   rewrite assign_seq_lt; try lia.
   rewrite Heqe. simpl.
   unfold nor_mode,turn_rqft.
-  rewrite assign_seq_out; easy. 
+  assert (nor_mode f c).
+  apply type_nor_mode with (aenv := aenv) (env := tenv); try easy.
+  rewrite assign_seq_out; easy.
 Qed.
 
-Lemma qft_acu_sem : forall l tenv tenv' aenv f x c size, phi_modes f x (S size) -> aenv x = S size
-          -> nor_mode f c -> fst c <> x ->
-          well_typed_pexp aenv l tenv (RQFT x) l tenv' -> right_mode_env aenv tenv f ->
-           qft_uniform aenv tenv f -> qft_gt aenv tenv f ->
-                  well_formed_ls l -> exp_neu_prop l ->
-          prog_sem aenv (qft_acu x c) f = f[c |-> put_cu (f c) ((¬ (get_r_qft f x 0)) ⊕ get_cua (f c))].
+Lemma qft_acu_sem : forall tenv aenv f x c size,
+            aenv x = S size -> fst c <> x -> Env.MapsTo x (Phi (aenv x)) tenv -> 
+            Env.MapsTo (fst c) Nor tenv -> snd c < aenv (fst c) ->
+             right_mode_env aenv tenv f -> qft_uniform aenv tenv f -> qft_gt aenv tenv f ->
+           exp_sem aenv (qft_acu x c) f = f[c |-> put_cu (f c) ((¬ (get_r_qft f x 0)) ⊕ get_cua (f c))].
 Proof.
   intros.
   unfold qft_acu.
   remember (RQFT x) as e.
-  assert (QFT x = inv_pexp e). rewrite Heqe. simpl. easy.
-  rewrite H9. simpl.
+  assert (QFT x = inv_exp e). rewrite Heqe. simpl. easy.
+  rewrite H7. simpl.
   rewrite cnot_sem.
   destruct c.
   rewrite eupdate_index_eq.
@@ -1210,26 +992,27 @@ Proof.
   rewrite eupdate_index_neq by iner_p.
   rewrite eupdate_index_eq.
   rewrite eupdate_index_neq by iner_p.
-  assert (((prog_sem aenv e f) [(x, 0)
-    |-> exchange (exchange (prog_sem aenv e f (x, 0)))]) = (prog_sem aenv e f)).
+  assert (((exp_sem aenv e f) [(@pair var nat x O)
+    |-> exchange (exchange (exp_sem aenv e f (@pair var nat x O)))]) = (exp_sem aenv e f)).
   rewrite eupdate_same. easy.
   unfold exchange.
-  destruct (prog_sem aenv e f (x, 0)) eqn:eq1.
-  assert ((¬ (¬ b)) = b) by btauto. rewrite H10. 1-3:easy.
-  rewrite H10.
-  rewrite fresh_pexp_sem_out.
-  assert ((prog_sem aenv (inv_pexp e) (prog_sem aenv e f))
-          = prog_sem aenv (e ;; inv_pexp e) f). simpl. easy.
-  rewrite H11.
-  rewrite inv_pexp_correct_rev with (tenv := tenv) (tenv' := tenv') (l:=l) (l':=l); try easy.
+  destruct (exp_sem aenv e f (@pair var nat x O)) eqn:eq1.
+  assert ((¬ (¬ b)) = b) by btauto. rewrite H8. 1-3:easy.
+  rewrite H8.
+  rewrite efresh_exp_sem_out.
+  assert ((exp_sem aenv (inv_exp e) (exp_sem aenv e f))
+          = exp_sem aenv (e ; inv_exp e) f). simpl. easy.
+  rewrite H9.
+  rewrite inv_exp_correct_rev with (tenv := tenv) (tenv' := Env.add x Nor tenv); try easy.
   apply eupdate_same_1. easy.
   rewrite Heqe. simpl.
   unfold turn_rqft,turn_qft.
   rewrite assign_seq_out; try iner_p.
   rewrite assign_seq_lt; try lia.
   unfold exchange. unfold get_cua. easy.
-  rewrite Heqe. simpl. constructor.
-  unfold or_not_eq. left. lia.
+  rewrite Heqe. simpl. constructor. easy. easy.
+  subst. simpl. constructor.
+  unfold or_not_eq. left. easy.
   unfold nor_mode. rewrite eupdate_index_eq.
   rewrite Heqe. simpl.
   unfold turn_rqft.
@@ -1238,71 +1021,13 @@ Proof.
   simpl.
   unfold nor_mode,turn_rqft.
   rewrite eupdate_index_neq.
+  assert (nor_mode f c).
+  apply type_nor_mode with (aenv := aenv) (env := tenv); try easy.
   rewrite assign_seq_out; easy. destruct c. iner_p. 
 Qed.
 
-Lemma get_r_qft_out : forall x c v f, fst c <> x -> get_r_qft (f[c |-> v]) x = get_r_qft f x.
-Proof.
-  intros. unfold get_r_qft.
-  destruct c.
-  rewrite eupdate_index_neq by iner_p. easy.
-Qed.
-
-Lemma env_eq_well_typed : forall e tenv tenv', Env.Equal tenv tenv' 
-                 -> well_typed_exp tenv e -> well_typed_exp tenv' e.
-Proof.
- intros.
- induction H0. constructor.
- constructor.
- eapply mapsto_equal. apply H0. easy.
- apply x_had.
- eapply mapsto_equal. apply H0. easy.
- constructor.
- eapply mapsto_equal. apply H0. easy.
- apply IHwell_typed_exp. easy.
- constructor.
- eapply mapsto_equal. apply H0. easy.
- eapply mapsto_equal. apply H1. easy.
- constructor.
- eapply mapsto_equal. apply H0. easy.
- apply rz_had.
- eapply mapsto_equal. apply H0. easy.
- constructor.
- eapply mapsto_equal. apply H0. easy.
- apply rrz_had.
- eapply mapsto_equal. apply H0. easy.
- apply sr_had with (n:=n).
- eapply mapsto_equal. apply H0. easy. easy.
- apply srr_had with (n:=n).
- eapply mapsto_equal. apply H0. easy. easy.
- constructor.
- eapply mapsto_equal. apply H0. easy.
- apply lshift_had.
- eapply mapsto_equal. apply H0. easy.
- constructor.
- eapply mapsto_equal. apply H0. easy.
- apply rshift_had.
- eapply mapsto_equal. apply H0. easy.
- constructor.
- eapply mapsto_equal. apply H0. easy.
- apply rev_had.
- eapply mapsto_equal. apply H0. easy.
- constructor.
- apply IHwell_typed_exp1; easy.
- apply IHwell_typed_exp2; easy.
-Qed.
-
-Lemma env_eq_right_mode : forall tenv tenv' aenv f, Env.Equal tenv tenv'
-          -> right_mode_env aenv tenv f -> right_mode_env aenv tenv' f.
-Proof.
-  intros.
-  unfold right_mode_env in *. intros.
-  specialize (H0 t p H1).
-  apply mapsto_equal with (s2 := tenv) in H2. apply H0. easy.
-  apply EnvFacts.Equal_sym. easy.
-Qed.
-
-Lemma exp_neu_rz_adder' : forall n l x size A, exp_neu l (rz_adder' x n size A) l.
+(*
+Lemma exp_neu_rz_adder' : forall n l x size A, exp_neu_l l (rz_adder' x n size A) l.
 Proof.
   induction n; intros; try easy.
   constructor. 
@@ -1311,7 +1036,7 @@ Proof.
   destruct (A n). constructor. constructor.
 Qed.
 
-Lemma exp_neu_rz_sub' : forall n l x size A, exp_neu l (rz_sub' x n size A) l.
+Lemma exp_neu_rz_sub' : forall n l x size A, exp_neu_l l (rz_sub' x n size A) l.
 Proof.
   induction n; intros; try easy.
   constructor. 
@@ -1321,7 +1046,7 @@ Proof.
 Qed.
 
 Lemma exp_neu_rz_adder_sub : forall l x size A M,
-           exp_neu l (rz_adder x size A; rz_sub x size M) l.
+           exp_neu_l l (rz_adder x size A; rz_sub x size M) l.
 Proof.
   intros. econstructor.
   apply exp_neu_rz_adder'.
@@ -1350,17 +1075,13 @@ Proof.
   specialize (IHe1 l l' l'0 H4 H3). subst.
   apply IHe2 with (l := l'0). easy. easy.
 Qed.
-
-Lemma mod_adder_half_sem : forall size f x c A B M aenv l l' tenv tenv',
-         phi_modes f x (S size) -> aenv x = S size -> nor_mode f c -> fst c <> x ->
-         get_cua (f c) = false ->
-           exp_scope aenv x (S size) (rz_adder x (S size) (nat2fb A); rz_sub x (S size) (nat2fb M))
-        -> well_typed_pexp aenv l tenv (mod_adder_half x (S size) c (nat2fb A) (nat2fb M)) l' tenv'
-        -> right_mode_env aenv tenv f -> qft_uniform aenv tenv f -> qft_gt aenv tenv f
-        -> 1 < M < 2^size -> A < M -> B < M ->
-        fbrev (S size) (get_r_qft f x) = nat2fb B ->
-                  well_formed_ls l -> exp_neu_prop l ->
-      (get_r_qft (prog_sem aenv (mod_adder_half x (S size) c (nat2fb A) (nat2fb M)) f) x)
+*)
+Lemma mod_adder_half_sem : forall size f x c A B M aenv tenv,
+            aenv x = S size -> fst c <> x -> Env.MapsTo x (Phi (aenv x)) tenv -> 
+            Env.MapsTo (fst c) Nor tenv  -> get_cua (f c) = false -> snd c < aenv (fst c)
+            -> 1 < M < 2^size -> A < M -> B < M -> fbrev (S size) (get_r_qft f x) = nat2fb B
+            -> right_mode_env aenv tenv f -> qft_uniform aenv tenv f -> qft_gt aenv tenv f ->
+      (get_r_qft (exp_sem aenv (mod_adder_half x (S size) c (nat2fb A) (nat2fb M)) f) x)
            = (fbrev (S size) (nat2fb (((B + A) mod M)))).
 Proof.
   intros.
@@ -1373,15 +1094,16 @@ Proof.
   assert (get_r_qft g x = 
        fbrev (S size) (nat2fb ((B + A + 2 ^ S size - M) mod 2 ^ S size))).
   subst.
-  inv H5. inv H19. inv H18. inv H20. inv H22. inv H4. inv H15. inv H16.
-  rewrite adder_sub_seq with (B := B) (tenv:=env'0) ; try easy.
+  rewrite adder_sub_seq with (B := B) (tenv:=tenv) ; try easy.
   1-3:simpl;lia.
-  inv H5. inv H20. inv H24. inv H20. inv H26.
-  remember (rz_adder x (S size) (nat2fb A);
-            rz_sub x (S size) (nat2fb M)) as e1.
-  rewrite qft_cu_sem with (tenv := env'0) (tenv' := env'1) (size := size) (l:=l'1); try easy.
-  rewrite efresh_exp_sem_irrelevant.
-  rewrite H3. bt_simpl. rewrite H15.
+  Check qft_cu_sem.
+  rewrite qft_cu_sem with (tenv := tenv) (size := size); try easy.
+  assert ((g c) = f c). subst.
+  rewrite efresh_exp_sem_irrelevant. easy.
+  constructor. apply efresh_rz_adder; easy.
+  apply efresh_rz_sub;easy.
+  rewrite H13.
+  rewrite H3. bt_simpl. rewrite H12.
   rewrite highbit_means_lt with (X := B + A) (M := M) ; try (simpl;lia).
   unfold one_cu_adder.
   Local Opaque rz_adder. 
@@ -1392,8 +1114,7 @@ Proof.
   bdestruct (B + A <? M).
   rewrite efresh_exp_sem_out; try (apply efresh_rz_adder; try easy).
   rewrite get_r_qft_out; try easy.
-  inv H23. inv H28.
-  rewrite rz_adder_full with (A:= ((B + A + 2 ^ S size - M) mod 2 ^ S size)) (tenv:= tenv'); try easy.
+  rewrite rz_adder_full with (A:= ((B + A + 2 ^ S size - M) mod 2 ^ S size)) (tenv:= tenv); try easy.
   assert (2^S size <> 0).
   apply Nat.pow_nonzero; lia.
   rewrite Nat.add_mod by lia.
@@ -1401,46 +1122,27 @@ Proof.
   rewrite <- Nat.add_mod by lia.
   assert (M < 2^S size) by (simpl;lia).
   assert (B + A + 2 ^ S size - M + M = B + A + 2^S size) by lia.
-  rewrite H26.
+  rewrite H17.
   rewrite Nat.add_mod by lia.
   rewrite Nat.mod_same by lia.
   rewrite plus_0_r.
   rewrite Nat.mod_mod by lia.
   rewrite Nat.mod_small by lia.
   rewrite Nat.mod_small by lia. easy.
-  apply phi_modes_exp; try easy.
-  inv H19. inv H21. inv H25.
-  assert (Env.Equal env'0 tenv').
-  apply EnvFacts.Equal_trans with (m' := (Env.add x (Phi (aenv x)) env'1)).
-  apply EnvFacts.Equal_trans with (m' := (Env.add x (Phi (aenv x)) ((Env.add x Nor env'0)))).
-  unfold Env.Equal. intros.
-  bdestruct (x =? y). subst.
-  rewrite find_add.
-  apply Env.find_1 in H19. easy.
-  repeat rewrite EnvFacts.add_neq_o by lia.
-  easy.
-  unfold Env.Equal. intros.
-  bdestruct (x =? y). subst.
-  rewrite find_add.
-  rewrite find_add. easy.
-  rewrite EnvFacts.add_neq_o by lia.
-  apply EnvFacts.Equal_sym in H33.
-  unfold Env.Equal in H33.
-  rewrite EnvFacts.add_neq_o with (m := env'1) by lia. easy.
-  apply EnvFacts.Equal_sym. easy.
-  apply well_typed_right_mode_exp; try easy.
-  apply env_eq_well_typed with (tenv := env'0). easy.
-  easy.
-  apply env_eq_right_mode with (tenv := env'0). easy. easy.
+  subst. 
+  apply well_typed_right_mode_pexp with (tenv := tenv).
+  apply pe_seq with (env' := tenv).
+  apply rz_adder_well_typed; try easy.
+  apply rz_sub_well_typed; try easy. easy.
   simpl. lia.
   apply Nat.mod_upper_bound.
   apply Nat.pow_nonzero ; lia.
-  rewrite H15.
+  rewrite H12.
   rewrite fbrev_twice_same. easy.
   rewrite get_r_qft_out by easy.
-  rewrite H15.
+  rewrite H12.
   assert ((B + A + 2 ^ S size - M) = (B + A - M) + 2^S size) by lia.
-  rewrite H18.
+  rewrite H15.
   assert (2^S size <> 0).
   apply Nat.pow_nonzero; lia.
   rewrite Nat.add_mod by lia.
@@ -1458,33 +1160,30 @@ Proof.
     }
   replace (M * ((B + A) / M)) with M by nia.
   easy.
-  subst. constructor. apply efresh_rz_adder; easy.
-  apply efresh_rz_sub; easy.
-  apply phi_modes_exp. subst. easy. easy.
-  unfold nor_mode.
-  rewrite efresh_exp_sem_irrelevant. apply H1.
-  subst. constructor. apply efresh_rz_adder; easy.
-  apply efresh_rz_sub; easy. inv H21. constructor; try easy.
-  apply well_typed_right_mode_exp; try easy.
-  inv H19. easy. inv H19. easy.
-  inv H19.
-  apply qft_uniform_exp_trans; try easy.
-  inv H19. apply qft_gt_exp_trans; try easy.
-  subst. inv H19.
-  specialize (exp_neu_rz_adder_sub l x (S size) (nat2fb A) (nat2fb M)) as eq5.
-  apply exp_neu_same with (l1 := l'1)  in eq5. subst. easy. easy.
-  inv H19.
-  specialize (exp_neu_rz_adder_sub l x (S size) (nat2fb A) (nat2fb M)) as eq5.
-  apply exp_neu_same with (l1 := l'1)  in eq5. subst. easy. easy.
+  apply type_nor_mode with (aenv := aenv) (env := tenv); try easy.
+  subst.
+  apply well_typed_right_mode_pexp with (tenv := tenv); try easy.
+  apply pe_seq with (env' := tenv).
+  apply rz_adder_well_typed; try easy.
+  apply rz_sub_well_typed; try easy.
+  subst.
+  apply qft_uniform_exp_trans with (tenv := tenv); try easy.
+  apply pe_seq with (env' := tenv).
+  apply rz_adder_well_typed; try easy.
+  apply rz_sub_well_typed; try easy.
+  subst.
+  apply qft_gt_exp_trans with (tenv := tenv); try easy.
+  apply pe_seq with (env' := tenv).
+  apply rz_adder_well_typed; try easy.
+  apply rz_sub_well_typed; try easy.
 Qed.
 
-Lemma clean_hbit_sem: forall size f x c B A aenv l tenv tenv', 
-         phi_modes f x (S size) -> aenv x = S size -> nor_mode f c -> fst c <> x ->
-         well_typed_pexp aenv l tenv (Exp (rz_sub x (S size) (nat2fb A))) l tenv -> right_mode_env aenv tenv f ->
-         A < 2^ size -> B < 2^size -> qft_uniform aenv tenv f -> qft_gt aenv tenv f ->
-         fbrev (S size) (get_r_qft f x) = nat2fb B -> well_typed_pexp aenv l tenv (RQFT x) l tenv' ->
-                  well_formed_ls l -> exp_neu_prop l ->
-        prog_sem aenv (clean_hbit x (S size) c (nat2fb A)) f =
+Lemma clean_hbit_sem: forall size f x c B A aenv tenv, 
+            aenv x = S size -> fst c <> x -> Env.MapsTo x (Phi (aenv x)) tenv -> 
+            Env.MapsTo (fst c) Nor tenv -> snd c < aenv (fst c)
+            -> A < 2^ size -> B < 2^size -> fbrev (S size) (get_r_qft f x) = nat2fb B
+            -> right_mode_env aenv tenv f -> qft_uniform aenv tenv f -> qft_gt aenv tenv f ->
+        exp_sem aenv (clean_hbit x (S size) c (nat2fb A)) f =
                 f[c |-> put_cu (f c) ((¬ (fbrev (S size)
                            (nat2fb ((B + 2^S size - A) mod 2^S size)) 0)) ⊕ get_cua (f c))].
 Proof.
@@ -1492,42 +1191,34 @@ Proof.
   Local Opaque rz_sub qft_acu. simpl.
   Local Transparent rz_sub qft_acu.
   assert (A < 2^ S size) by (simpl;lia).
-  assert (B < 2^ S size) by (simpl;lia). inv H3.
-  specialize (rz_sub_full (S size) f x B A aenv tenv H H20 H4 H13 H14 H9) as eq1.
-  rewrite qft_acu_sem with (tenv := tenv) (tenv' := tenv') (size := size) (l:=l); try easy.
+  assert (B < 2^ S size) by (simpl;lia).
+  assert (S size = aenv x) as X1 by lia.
+  specialize (rz_sub_full (S size) f x B A aenv tenv X1 H1 H7 H10 H11 H6) as eq1.
+  rewrite qft_acu_sem with (tenv := tenv) (size := size); try easy.
   rewrite efresh_exp_sem_out.
   assert ((exp_sem aenv (inv_exp (rz_sub x (S size) (nat2fb A)))
    (exp_sem aenv (rz_sub x (S size) (nat2fb A)) f))
    = exp_sem aenv (rz_sub x (S size) (nat2fb A) ; inv_exp (rz_sub x (S size) (nat2fb A))) f).
   easy.
-  rewrite H3. clear H3.
-  rewrite inv_exp_correct_rev with (tenv := tenv); try easy.
+  rewrite H12. clear H12.
+  rewrite inv_exp_correct_rev with (tenv := tenv) (tenv' := tenv); try easy.
   apply eupdate_same_1. easy.
   rewrite eq1.
   rewrite efresh_exp_sem_irrelevant. simpl. easy.
-  apply efresh_rz_sub; try lia.
+  apply efresh_rz_sub; try lia. easy.
+  apply rz_sub_well_typed; try easy.
   apply fresh_inv_exp.
-  apply efresh_rz_sub; try lia.
-  apply phi_modes_exp.
-  apply escope_rz_sub. easy.
-  unfold nor_mode.
-  rewrite efresh_exp_sem_irrelevant. easy.
-  apply efresh_rz_sub; try lia.
-  apply well_typed_right_mode_exp; try easy.
-  apply qft_uniform_exp_trans; try easy.
-  apply qft_gt_exp_trans; try easy.
-Qed.
-
-Lemma put_cu_get_r : forall c f b, nor_mode f c -> put_cu (f c) b = nval b (get_r (f c)).
-Proof.
-  intros.
-  unfold put_cu, get_r.
-  unfold nor_mode in H.
-  destruct (f c). easy. lia. lia.
+  apply efresh_rz_sub; try lia. easy.
+  apply well_typed_right_mode_pexp with (tenv := tenv); try easy.
+  apply rz_sub_well_typed; try easy.
+  apply qft_uniform_exp_trans with (tenv := tenv); try easy.
+  apply rz_sub_well_typed; try easy.
+  apply qft_gt_exp_trans with (tenv := tenv); try easy.
+  apply rz_sub_well_typed; try easy.
 Qed.
 
 Lemma qft_cu_r_same : forall aenv x c f, nor_mode f c -> fst c <> x -> 0 < aenv x ->
-             get_r ((prog_sem aenv (qft_cu x c) f) c) = get_r (f c).
+             get_r ((exp_sem aenv (qft_cu x c) f) c) = get_r (f c).
 Proof.
   intros. simpl.
   unfold turn_qft.
@@ -1566,7 +1257,7 @@ Proof.
 Qed.
 
 Lemma nor_mode_qft_cu : forall x aenv f p, nor_mode f p -> fst p <> x -> 0 < aenv x ->
-                nor_mode (prog_sem aenv (qft_cu x p) f) p.
+                nor_mode (exp_sem aenv (qft_cu x p) f) p.
 Proof.
   intros.
   unfold nor_mode in *.
@@ -1586,7 +1277,7 @@ Proof.
 Qed.
 
 Lemma nor_mode_qft_acu : forall x aenv f p, nor_mode f p -> fst p <> x -> 0 < aenv x ->
-                nor_mode (prog_sem aenv (qft_acu x p) f) p.
+                nor_mode (exp_sem aenv (qft_acu x p) f) p.
 Proof.
   intros.
   unfold nor_mode in *.
@@ -1614,7 +1305,7 @@ Qed.
 
 
 Lemma nor_mode_mod_adder : forall x n c aenv f A M, phi_modes f x n -> 
-          nor_mode f c -> fst c <> x -> 0 < aenv x -> nor_mode (prog_sem aenv (mod_adder x n c A M) f) c.
+          nor_mode f c -> fst c <> x -> 0 < aenv x -> nor_mode (exp_sem aenv (mod_adder x n c A M) f) c.
 Proof.
   intros.
   unfold mod_adder,mod_adder_half,clean_hbit.
@@ -1642,7 +1333,7 @@ Qed.
 
 
 Lemma phi_modes_qft_cu : forall x n c aenv f, phi_modes f x n -> 
-          nor_mode f c -> fst c <> x -> 0 < aenv x -> phi_modes (prog_sem aenv (qft_cu x c) f) x n.
+          nor_mode f c -> fst c <> x -> 0 < aenv x -> phi_modes (exp_sem aenv (qft_cu x c) f) x n.
 Proof. 
   intros.
   unfold phi_modes in *.
@@ -1676,7 +1367,7 @@ Proof.
 Qed.
 
 Lemma phi_modes_qft_acu : forall x n c aenv f, phi_modes f x n -> 
-          nor_mode f c -> fst c <> x -> 0 < aenv x -> phi_modes (prog_sem aenv (qft_acu x c) f) x n.
+          nor_mode f c -> fst c <> x -> 0 < aenv x -> phi_modes (exp_sem aenv (qft_acu x c) f) x n.
 Proof. 
   intros.
   unfold phi_modes in *.
@@ -1737,7 +1428,7 @@ Proof.
 Qed.
 
 Lemma phi_modes_mod_adder : forall x n c aenv f A M, phi_modes f x n -> 
-          nor_mode f c -> fst c <> x -> 0 < aenv x -> phi_modes (prog_sem aenv (mod_adder x n c A M) f) x n.
+          nor_mode f c -> fst c <> x -> 0 < aenv x -> phi_modes (exp_sem aenv (mod_adder x n c A M) f) x n.
 Proof.
   intros.
   unfold mod_adder,mod_adder_half,clean_hbit.
@@ -1772,7 +1463,7 @@ Proof.
   apply efresh_rz_sub; try easy.
 Qed.
 
-
+(*
 Lemma exp_neu_qft_cu : forall l x c, pexp_neu l (qft_cu x c) l.
 Proof.
   intros.
@@ -1825,216 +1516,221 @@ Proof.
   constructor. constructor.
   Local Opaque CNOT.
 Qed.
+*)
 
-Lemma mod_adder_sem : forall size f x c A B M aenv l l' tenv tenv',
-         phi_modes f x (S size) -> aenv x = S size -> nor_mode f c -> fst c <> x ->
-         get_cua (f c) = false
-        -> well_typed_pexp aenv l tenv (mod_adder x (S size) c (nat2fb A) (nat2fb M)) l' tenv'
-        -> right_mode_env aenv tenv f -> qft_uniform aenv tenv f -> qft_gt aenv tenv f
-        -> 1 < M < 2^size -> A < M -> B < M ->
-        fbrev (S size) (get_r_qft f x) = nat2fb B ->
-                  well_formed_ls l -> exp_neu_prop l ->
-      (get_r_qft (prog_sem aenv (mod_adder x (S size) c (nat2fb A) (nat2fb M)) f) x)
+Lemma exp_neu_rz_adder : forall n x y size M, n <= size -> exp_neu_l y [] (rz_adder' x n size M) [].
+Proof.
+ induction n;intros;simpl. constructor.
+ apply seq_neul with (l' := []).
+ apply IHn. lia.
+ destruct (M n). constructor. constructor.
+Qed.
+
+Lemma mod_adder_half_well_typed : forall x c size A M aenv tenv,
+            aenv x = size -> fst c <> x -> Env.MapsTo x (Phi (aenv x)) tenv -> Env.MapsTo (fst c) Nor tenv
+          -> well_typed_pexp aenv tenv (mod_adder_half x size c A M) tenv.
+Proof.
+ intros. unfold mod_adder_half.
+ apply pe_seq with (env' := tenv).
+ apply pe_seq with (env' := tenv).
+ apply pe_seq with (env' := tenv).
+ apply rz_adder_well_typed; try easy.
+ apply rz_sub_well_typed; try easy.
+ unfold qft_cu.
+ apply pe_seq with (env' := Env.add x Nor tenv).
+ apply pe_seq with (env' := Env.add x Nor tenv).
+ apply rqft_phi. easy.
+ easy.
+ apply cnot_wt_nor; try easy. destruct c. iner_p.
+ simpl. apply Env.add_1. easy.
+ simpl. apply Env.add_2. iner_p. easy.
+ apply qft_nor. apply Env.add_1. easy.
+ apply EnvFacts.Equal_mapsto_iff.
+ intros. split. intros.
+ bdestruct (k =? x). subst.
+ apply mapsto_always_same with (v2 := e) in H1. subst.
+ apply Env.add_1. easy. easy.
+ apply Env.add_2. lia. apply Env.add_2. lia. easy.
+ intros.
+ bdestruct (k =? x). subst. 
+ apply mapsto_add1 in H3. subst. easy.
+ apply Env.add_3 in H3. apply Env.add_3 in H3. easy. lia. lia.
+ unfold one_cu_adder.
+ apply pcu_nor; try easy.
+ apply efresh_rz_adder; try easy.
+ simpl.
+ unfold exp_neu. intros.
+ apply exp_neu_rz_adder. easy.
+ apply rz_adder_well_typed; try easy.
+Qed.
+
+Lemma mod_adder_well_typed : forall x c size A M aenv tenv,
+            aenv x = size -> fst c <> x -> Env.MapsTo x (Phi (aenv x)) tenv -> Env.MapsTo (fst c) Nor tenv
+          -> well_typed_pexp aenv tenv (mod_adder x size c A M) tenv.
+Proof.
+ intros. unfold mod_adder,mod_adder_half,clean_hbit.
+ apply pe_seq with (env' := tenv).
+ apply pe_seq with (env' := tenv).
+ apply pe_seq with (env' := tenv).
+ apply pe_seq with (env' := tenv).
+ apply rz_adder_well_typed; try easy.
+ apply rz_sub_well_typed; try easy.
+ unfold qft_cu.
+ apply pe_seq with (env' := Env.add x Nor tenv).
+ apply pe_seq with (env' := Env.add x Nor tenv).
+ apply rqft_phi. easy.
+ easy.
+ apply cnot_wt_nor; try easy. destruct c. iner_p.
+ simpl. apply Env.add_1. easy.
+ simpl. apply Env.add_2. iner_p. easy.
+ apply qft_nor. apply Env.add_1. easy.
+ apply EnvFacts.Equal_mapsto_iff.
+ intros. split. intros.
+ bdestruct (k =? x). subst.
+ apply mapsto_always_same with (v2 := e) in H1. subst.
+ apply Env.add_1. easy. easy.
+ apply Env.add_2. lia. apply Env.add_2. lia. easy.
+ intros.
+ bdestruct (k =? x). subst. 
+ apply mapsto_add1 in H3. subst. easy.
+ apply Env.add_3 in H3. apply Env.add_3 in H3. easy. lia. lia.
+ unfold one_cu_adder.
+ apply pcu_nor; try easy.
+ apply efresh_rz_adder; try easy.
+ simpl.
+ unfold exp_neu. intros.
+ apply exp_neu_rz_adder. easy.
+ apply rz_adder_well_typed; try easy.
+ apply pe_seq with (env' := tenv).
+ apply pe_seq with (env' := tenv).
+ apply rz_sub_well_typed; try easy.
+ unfold qft_acu.
+ apply pe_seq with (env' := Env.add x Nor tenv).
+ apply pe_seq with (env' := Env.add x Nor tenv).
+ apply rqft_phi. easy. easy.
+ apply pe_seq with (env' := Env.add x Nor tenv).
+ apply pe_seq with (env' := Env.add x Nor tenv).
+ constructor. constructor. simpl. apply Env.add_1. easy.
+ apply cnot_wt_nor. destruct c. iner_p.
+ simpl. apply Env.add_1. easy.
+ apply Env.add_2. iner_p. easy.
+ constructor. constructor. simpl. apply Env.add_1. easy.
+ apply qft_nor. apply Env.add_1. easy.
+ apply EnvFacts.Equal_mapsto_iff.
+ intros. split. intros.
+ bdestruct (k =? x). subst.
+ apply mapsto_always_same with (v2 := e) in H1. subst.
+ apply Env.add_1. easy. easy.
+ apply Env.add_2. lia. apply Env.add_2. lia. easy.
+ intros.
+ bdestruct (k =? x). subst. 
+ apply mapsto_add1 in H3. subst. easy.
+ apply Env.add_3 in H3. apply Env.add_3 in H3. easy. lia. lia.
+ apply typed_inv_pexp.
+ apply rz_sub_well_typed; try easy.
+Qed.
+
+Lemma mod_adder_sem : forall size f x c A B M aenv tenv,
+            aenv x = S size -> fst c <> x -> Env.MapsTo x (Phi (aenv x)) tenv -> 
+            Env.MapsTo (fst c) Nor tenv  -> get_cua (f c) = false -> snd c < aenv (fst c)
+            -> 1 < M < 2^size -> A < M -> B < M -> fbrev (S size) (get_r_qft f x) = nat2fb B
+            -> right_mode_env aenv tenv f -> qft_uniform aenv tenv f -> qft_gt aenv tenv f ->
+      (get_r_qft (exp_sem aenv (mod_adder x (S size) c (nat2fb A) (nat2fb M)) f) x)
            = (fbrev (S size) (nat2fb (((B + A) mod M)))).
 Proof.
   intros.
   Local Opaque mod_adder_half clean_hbit. simpl.
-  inv H4.
   Local Transparent mod_adder_half clean_hbit.
   assert (exp_scope aenv x (S size)
         (rz_adder x (S size) (nat2fb A); rz_sub x (S size) (nat2fb M))).
   constructor. apply escope_rz_adder. apply escope_rz_sub.
   Check mod_adder_half_sem.
-  specialize (mod_adder_half_sem size f x c A B M aenv l l'0 tenv env'
-                 H H0 H1 H2 H3 H4 H18 H5 H6 H7 H8 H9 H10 H11 H12 H13) as eq1.
-  unfold clean_hbit in H21. inv H21. inv H19. inv H20. unfold qft_acu in H24. inv H24. inv H22.
+  specialize (mod_adder_half_sem size f x c A B M aenv tenv
+              H H0 H1 H2 H3 H4 H5 H6 H7 H8 H9 H10 H11) as eq1.
   Check clean_hbit_sem.
-  rewrite clean_hbit_sem with (tenv := env'1)
-        (tenv' := env'2) (B:=((B + A) mod M)) (l := l'2); try easy.
+  rewrite clean_hbit_sem with (tenv := tenv) (B:=((B + A) mod M)); try easy.
   rewrite get_r_qft_out by easy.
-  rewrite eq1. easy.
-  unfold mod_adder_half.
-  remember (rz_adder x (S size) (nat2fb A); rz_sub x (S size) (nat2fb M)) as e1.
-  Local Opaque qft_cu one_cu_adder.
-  simpl.
-  Local Transparent qft_cu one_cu_adder.
-  apply phi_modes_exp.
-  unfold one_cu_adder. constructor.
-  apply escope_rz_adder.
-  apply phi_modes_qft_cu ; try easy.
-  apply phi_modes_exp. subst.
-  constructor. apply escope_rz_adder.
-  apply escope_rz_sub. easy.
-  unfold nor_mode.
-  rewrite efresh_exp_sem_irrelevant. apply H1.
-  subst. constructor.
-  apply efresh_rz_adder. easy. lia.
-  apply efresh_rz_sub. easy. lia. lia.
-  unfold nor_mode.
-  unfold mod_adder_half.
-  remember (rz_adder x (S size) (nat2fb A); rz_sub x (S size) (nat2fb M)) as e1.
-  unfold one_cu_adder.
-  Local Opaque qft_cu rz_adder.
-  simpl.
-  Local Transparent qft_cu rz_adder.
-  destruct (get_cua (prog_sem aenv (qft_cu x c) (exp_sem aenv e1 f) c)).
-  rewrite efresh_exp_sem_irrelevant.
-  unfold qft_cu. simpl.
-  unfold turn_qft.
-  rewrite assign_r_out by iner_p.
-  rewrite cnot_sem.
-  rewrite eupdate_index_eq.
-  unfold turn_rqft.
-  rewrite assign_seq_out by easy.
-  rewrite Heqe1.
-  rewrite efresh_exp_sem_irrelevant.
-  unfold nor_mode in H1. destruct (f c).
-  unfold put_cu. 1-3:lia.
-  constructor.
-  apply efresh_rz_adder. easy. lia.
-  apply efresh_rz_sub. easy. lia.
-  unfold nor_mode.
-  unfold turn_rqft. rewrite assign_seq_lt by lia. easy.
-  unfold nor_mode.
-  unfold turn_rqft. rewrite assign_seq_out by lia.
-  rewrite efresh_exp_sem_irrelevant. apply H1.
-  subst. constructor.
-  apply efresh_rz_adder. easy. lia.
-  apply efresh_rz_sub. easy. lia.
-  apply efresh_rz_adder. easy. lia.
-  unfold qft_cu. simpl.
-  unfold turn_qft.
-  rewrite assign_r_out by easy.
-  rewrite cnot_sem.
-  rewrite eupdate_index_eq.
-  unfold turn_rqft. rewrite assign_seq_out by easy.
-  rewrite efresh_exp_sem_irrelevant.
-  unfold nor_mode in H1. unfold put_cu.
-  destruct (f c). 1-3:lia.
-  subst. constructor.
-  apply efresh_rz_adder. easy. lia.
-  apply efresh_rz_sub. easy. lia.
-  unfold nor_mode.
-  unfold turn_rqft.
-  rewrite assign_seq_lt; lia.
-  unfold nor_mode.
-  unfold turn_rqft.
-  rewrite assign_seq_out by easy.
-  rewrite efresh_exp_sem_irrelevant. apply H1.
-  subst. constructor.
-  apply efresh_rz_adder. easy. lia.
-  apply efresh_rz_sub. easy. lia.
-  constructor. easy.
-  apply exp_neu_rz_sub'. easy. 
-  apply well_typed_right_mode_pexp with (tenv := tenv) (l := l) (l' := l'0); try easy.
-  lia.
+  rewrite eq1. easy. lia.
   assert ((B + A) mod M < M). 
   apply Nat.mod_upper_bound. lia. lia.
-  apply qft_uniform_pexp_trans with (tenv := tenv) (l := l) (l' := l'0); try easy.
-  apply qft_gt_pexp_trans with (tenv := tenv) (l := l) (l' := l'0); try easy.
   rewrite eq1.
   rewrite fbrev_twice_same. easy.
-  inv H24. constructor; try easy.
-  eapply exp_neu_well_formed_ls. apply H16.
-  eapply typed_pexp_well_formed_ls.
-  apply H18. easy.
-  eapply exp_neu_t_prop. apply H16.
-  eapply typed_pexp_well_formed_ls.
-  apply H18. easy.
-  eapply typed_pexp_neu_prop.
-  apply H18. easy. easy.
+  apply well_typed_right_mode_pexp with (tenv := tenv).
+  apply mod_adder_half_well_typed; try easy. easy.
+  apply qft_uniform_exp_trans with (tenv := tenv). easy.
+  apply mod_adder_half_well_typed; try easy. easy.
+  apply qft_gt_exp_trans with (tenv := tenv). easy.
+  apply mod_adder_half_well_typed; try easy. easy.
 Qed.
 
-
-Lemma mod_adder_half_high : forall size f x c A B M aenv l l' tenv tenv',
-         phi_modes f x (S size) -> aenv x = S size -> nor_mode f c -> fst c <> x ->
-         get_cua (f c) = false ->
-           exp_scope aenv x (S size) (rz_adder x (S size) (nat2fb A); rz_sub x (S size) (nat2fb M))
-        -> well_typed_pexp aenv l tenv (mod_adder_half x (S size) c (nat2fb A) (nat2fb M)) l' tenv'
-        -> right_mode_env aenv tenv f -> qft_uniform aenv tenv f -> qft_gt aenv tenv f
-        -> 1 < M < 2^size -> A < M -> B < M ->
-        fbrev (S size) (get_r_qft f x) = nat2fb B ->
-                  well_formed_ls l -> exp_neu_prop l ->
-      get_cua ((prog_sem aenv (mod_adder_half x (S size) c (nat2fb A) (nat2fb M)) f) c) = (B + A <? M).
+Lemma mod_adder_half_high : forall size f x c A B M aenv tenv,
+            aenv x = S size -> fst c <> x -> Env.MapsTo x (Phi (aenv x)) tenv -> 
+            Env.MapsTo (fst c) Nor tenv  -> get_cua (f c) = false -> snd c < aenv (fst c)
+            -> 1 < M < 2^size -> A < M -> B < M -> fbrev (S size) (get_r_qft f x) = nat2fb B
+            -> right_mode_env aenv tenv f -> qft_uniform aenv tenv f -> qft_gt aenv tenv f ->
+      get_cua ((exp_sem aenv (mod_adder_half x (S size) c (nat2fb A) (nat2fb M)) f) c) = (B + A <? M).
 Proof.
   intros.
   unfold mod_adder_half,qft_cu.
-  unfold qft_cu.
-  assert (prog_sem aenv
-     (((rz_adder x (S size) (nat2fb A); rz_sub x (S size) (nat2fb M));;
-       ((RQFT x;; CNOT (x, 0) c);; QFT x));;
+  assert (exp_sem aenv
+     (((rz_adder x (S size) (nat2fb A); rz_sub x (S size) (nat2fb M));
+       ((RQFT x; CNOT (@pair var nat x O) c); QFT x));
       one_cu_adder x (S size) c (nat2fb M)) f
-      = (prog_sem aenv
-        (Exp (rz_adder x (S size) (nat2fb A));; rz_compare_half x (S size) c M ;;
-          QFT x ;; one_cu_adder x (S size) c (nat2fb M)) f)).
+      = (exp_sem aenv
+        ( (rz_adder x (S size) (nat2fb A)); rz_compare_half x (S size) c M ;
+          QFT x ; one_cu_adder x (S size) c (nat2fb M)) f)).
   simpl. easy.
-  rewrite H15.
+  rewrite H12.
   Local Opaque rz_compare_half rz_adder.
   simpl.
   Local Transparent rz_compare_half rz_adder.
-  inv H5. inv H20. inv H19. inv H21. inv H23. inv H26.
   assert (A < 2 ^ S size) by (simpl;lia).
   assert (B < 2 ^ S size) by (simpl;lia).
   Check rz_adder_full.
-  specialize (rz_adder_full (S size) f x B A aenv env'0 H H20 H6 H5 H21 H12) as eq1.
+  assert (S size = aenv x) as X1 by easy.
+  specialize (rz_adder_full (S size) f x B A aenv tenv X1 H1 H9 H13 H14 H8) as eq1.
   unfold turn_qft.
   rewrite assign_r_out by easy.
   assert (get_cua
-       (prog_sem aenv (rz_compare_half x (S size) c M)
+       (exp_sem aenv (rz_compare_half x (S size) c M)
           (exp_sem aenv (rz_adder x (S size) (nat2fb A)) f) c) = (B + A <? M)).
   Check rz_compare_half_sem.
-  inv H24. inv H30.
-  rewrite rz_compare_half_sem with (A:=(B + A))
-          (tenv := env'0) (tenv' := env'1) (l := l'1) (l' := l'3); try easy.
-  apply phi_modes_exp. apply escope_rz_adder. easy.
-  unfold nor_mode.
-  rewrite efresh_exp_sem_irrelevant. apply H1.
-  apply efresh_rz_adder. easy. lia.
+  rewrite rz_compare_half_sem with (A:=(B + A)) (tenv := tenv); try easy.
   rewrite efresh_exp_sem_irrelevant. easy.
   apply efresh_rz_adder. easy. lia.
-  inv H16. inv H17.
-  unfold rz_compare_half. econstructor.
-  econstructor. constructor. easy.
-  apply exp_neu_rz_sub'.
-  easy. apply H29. constructor.
-  inv H34. easy. apply exp_neu_cnot. inv H34. easy.
-  apply well_typed_right_mode_exp; try easy.
+  apply well_typed_right_mode_pexp with (tenv := tenv); try easy.
+  apply rz_adder_well_typed; try easy.
   simpl. lia. lia.
   rewrite eq1.
   rewrite fbrev_twice_same.
   rewrite Nat.mod_small by (simpl;lia). easy.
-  rewrite H23.
+  rewrite H15.
   bdestruct (B + A <? M).
   rewrite efresh_exp_sem_irrelevant.
   rewrite assign_r_out by easy.
-  rewrite H23. easy.
+  rewrite H15. easy.
   apply efresh_rz_adder. easy. lia.
   rewrite assign_r_out by easy.
-  rewrite H23. easy.
+  rewrite H15. easy.
 Qed.
 
 
-Lemma mod_adder_typed : forall size f x c A B M aenv l l' tenv tenv',
-         phi_modes f x (S size) -> aenv x = S size -> nor_mode f c -> fst c <> x ->
-         get_cua (f c) = false
-        -> well_typed_pexp aenv l tenv (mod_adder x (S size) c (nat2fb A) (nat2fb M)) l' tenv'
-        -> right_mode_env aenv tenv f -> qft_uniform aenv tenv f -> qft_gt aenv tenv f
-        -> 1 < M < 2^size -> A < M -> B < M ->
-        fbrev (S size) (get_r_qft f x) = nat2fb B ->
-                  well_formed_ls l -> exp_neu_prop l ->
-            (prog_sem aenv (mod_adder x (S size) c (nat2fb A) (nat2fb M)) f) c = f c.
+Lemma mod_adder_typed : forall size f x c A B M aenv tenv,
+            aenv x = S size -> fst c <> x -> Env.MapsTo x (Phi (aenv x)) tenv -> 
+            Env.MapsTo (fst c) Nor tenv  -> get_cua (f c) = false -> snd c < aenv (fst c)
+            -> 1 < M < 2^size -> A < M -> B < M -> fbrev (S size) (get_r_qft f x) = nat2fb B
+            -> right_mode_env aenv tenv f -> qft_uniform aenv tenv f -> qft_gt aenv tenv f ->
+            (exp_sem aenv (mod_adder x (S size) c (nat2fb A) (nat2fb M)) f) c = f c.
 Proof.
   intros.
   Local Opaque mod_adder_half clean_hbit. simpl.
-  inv H4.
   Local Transparent mod_adder_half clean_hbit.
-  inv H21. inv H17. inv H23. inv H17. inv H19.
-  rewrite clean_hbit_sem with (B:= (((B + A) mod M)))
-         (tenv:= env'1) (tenv':= env'3) (l := l'0); try easy.
+  assert (nor_mode f c) as X1.
+  apply type_nor_mode with (aenv := aenv) (env := tenv); easy.
+  rewrite clean_hbit_sem with (B:= (((B + A) mod M))) (tenv := tenv); try easy.
   rewrite eupdate_index_eq.
-  rewrite mod_adder_half_high with (B:=B) (tenv:=tenv) 
-          (tenv' := env'1) (l := l) (l' := l'0); try easy.
-  assert (forall b, put_cu (prog_sem aenv 
+  rewrite mod_adder_half_high with (B:=B) (tenv:=tenv) ; try easy.
+  assert (forall b, put_cu (exp_sem aenv 
            (mod_adder_half x (S size) c (nat2fb A) (nat2fb M)) f c) b = put_cu (f c) b).
   intros. unfold mod_adder_half in *.
   remember ((rz_adder x (S size) (nat2fb A); rz_sub x (S size) (nat2fb M))) as e1.
@@ -2043,7 +1739,7 @@ Proof.
   rewrite one_cu_adder_r_same by easy.
   rewrite qft_cu_r_same ; try easy.
   rewrite efresh_exp_sem_irrelevant.
-  unfold nor_mode in H1.
+  unfold nor_mode in X1.
   destruct (f c). unfold get_r.
   unfold get_cua in H3. subst.
   unfold put_cu. easy. lia. lia.
@@ -2051,7 +1747,7 @@ Proof.
   apply efresh_rz_adder. easy. lia.
   apply efresh_rz_sub. easy. lia.
   unfold nor_mode.
-  rewrite efresh_exp_sem_irrelevant. apply H1.
+  rewrite efresh_exp_sem_irrelevant. apply X1.
   subst. constructor.
   apply efresh_rz_adder. easy. lia.
   apply efresh_rz_sub. easy. lia. lia.
@@ -2059,15 +1755,15 @@ Proof.
   apply nor_mode_one_cu_adder; try easy.
   apply nor_mode_qft_cu; try lia.
   unfold nor_mode. subst.
-  rewrite efresh_exp_sem_irrelevant. apply H1.
+  rewrite efresh_exp_sem_irrelevant. apply X1.
   constructor.
   apply efresh_rz_adder. easy. lia.
-  apply efresh_rz_sub. easy. lia.
-  rewrite H4.
+  apply efresh_rz_sub. easy. lia. easy.
+  rewrite H12.
   bdestruct (B + A <? M).
   rewrite (Nat.mod_small (B+A)) by lia.
   assert ((B + A + 2 ^ S size - A) = B + 2^S size) by lia.
-  rewrite H17.
+  rewrite H14.
   rewrite Nat.add_mod by (simpl;lia).
   rewrite Nat.mod_same by (simpl;lia). rewrite plus_0_r.
   rewrite Nat.mod_mod by (simpl;lia).
@@ -2075,124 +1771,43 @@ Proof.
   unfold fbrev. bdestruct (0 <? S size).
   simpl.
   assert ((size - 0 - 0) = size) by lia.
-  rewrite H23.
+  rewrite H16.
   unfold nat2fb.
   rewrite N2fb_Ntestbit. rewrite Ntestbit_lt_pow2n. simpl.
-  unfold put_cu. unfold get_cua in H3. unfold nor_mode in H1.
+  unfold put_cu. unfold get_cua in H3. unfold nor_mode in X1.
   destruct (f c). subst. easy. lia. lia.
-  assert (N.of_nat B < N.of_nat (2^size))%N by lia. simpl in H26.
-  rewrite Nofnat_pow in H26. simpl in H26. easy. lia.
-  specialize (mod_sum_lt A B M H9 H10) as eq2.
+  assert (N.of_nat B < N.of_nat (2^size))%N by lia. simpl in H17.
+  rewrite Nofnat_pow in H17. simpl in H17. easy. lia.
+  specialize (mod_sum_lt A B M H6 H7) as eq2.
   rewrite highbit_means_lt; try lia.
   rewrite plus_comm.
   bdestruct ((A + B) mod M <? A). 
   simpl. 
-  unfold put_cu. unfold get_cua in H3. unfold nor_mode in H1.
+  unfold put_cu. unfold get_cua in H3. unfold nor_mode in X1.
   destruct (f c). subst. easy. lia. lia.
-  rewrite plus_comm in H16.
-  apply eq2 in H16. lia.
+  rewrite plus_comm in H13.
+  apply eq2 in H13. lia.
   assert ((B + A) mod M < M) by (apply Nat.mod_upper_bound;lia).
   simpl. lia.
   rewrite plus_comm.
   assert ((A + B) mod M < A). apply eq2. lia.
-  lia.
-  constructor.
-  apply escope_rz_adder.
-  apply escope_rz_sub.
-  unfold mod_adder_half.
-  remember (rz_adder x (S size) (nat2fb A); rz_sub x (S size) (nat2fb M)) as e1.
-  Local Opaque qft_cu one_cu_adder.
-  simpl.
-  Local Transparent qft_cu one_cu_adder.
-  apply phi_modes_exp.
-  unfold one_cu_adder. constructor.
-  apply escope_rz_adder.
-  apply phi_modes_qft_cu ; try easy.
-  apply phi_modes_exp. subst.
-  constructor. apply escope_rz_adder.
-  apply escope_rz_sub. easy.
-  unfold nor_mode.
-  rewrite efresh_exp_sem_irrelevant. apply H1.
-  subst. constructor.
-  apply efresh_rz_adder. easy. lia.
-  apply efresh_rz_sub. easy. lia. lia.
-  unfold nor_mode.
-  unfold mod_adder_half.
-  remember (rz_adder x (S size) (nat2fb A); rz_sub x (S size) (nat2fb M)) as e1.
-  unfold one_cu_adder.
-  Local Opaque qft_cu rz_adder.
-  simpl.
-  Local Transparent qft_cu rz_adder.
-  destruct (get_cua (prog_sem aenv (qft_cu x c) (exp_sem aenv e1 f) c)).
-  rewrite efresh_exp_sem_irrelevant.
-  unfold qft_cu. simpl.
-  unfold turn_qft.
-  rewrite assign_r_out by iner_p.
-  rewrite cnot_sem.
-  rewrite eupdate_index_eq.
-  unfold turn_rqft.
-  rewrite assign_seq_out by easy.
-  rewrite Heqe1.
-  rewrite efresh_exp_sem_irrelevant.
-  unfold nor_mode in H1. destruct (f c).
-  unfold put_cu. 1-3:lia.
-  constructor.
-  apply efresh_rz_adder. easy. lia.
-  apply efresh_rz_sub. easy. lia.
-  unfold nor_mode.
-  unfold turn_rqft. rewrite assign_seq_lt by lia. easy.
-  unfold nor_mode.
-  unfold turn_rqft. rewrite assign_seq_out by lia.
-  rewrite efresh_exp_sem_irrelevant. apply H1.
-  subst. constructor.
-  apply efresh_rz_adder. easy. lia.
-  apply efresh_rz_sub. easy. lia.
-  apply efresh_rz_adder. easy. lia.
-  unfold qft_cu. simpl.
-  unfold turn_qft.
-  rewrite assign_r_out by easy.
-  rewrite cnot_sem.
-  rewrite eupdate_index_eq.
-  unfold turn_rqft. rewrite assign_seq_out by easy.
-  rewrite efresh_exp_sem_irrelevant.
-  unfold nor_mode in H1. unfold put_cu.
-  destruct (f c). 1-3:lia.
-  subst. constructor.
-  apply efresh_rz_adder. easy. lia.
-  apply efresh_rz_sub. easy. lia.
-  unfold nor_mode.
-  unfold turn_rqft.
-  rewrite assign_seq_lt; lia.
-  unfold nor_mode.
-  unfold turn_rqft.
-  rewrite assign_seq_out by easy.
-  rewrite efresh_exp_sem_irrelevant. apply H1.
-  subst. constructor.
-  apply efresh_rz_adder. easy. lia.
-  apply efresh_rz_sub. easy. lia.
-  constructor. easy. apply exp_neu_rz_sub'. easy.
-  apply well_typed_right_mode_pexp with (tenv := tenv) (l := l) (l' := l'0); try easy.
-  lia.
-  assert ((B + A) mod M < M). 
-  apply Nat.mod_upper_bound. lia. lia.
-  apply qft_uniform_pexp_trans with (tenv := tenv) (l := l) (l' := l'0); try easy.
-  apply qft_gt_pexp_trans with (tenv := tenv) (l := l) (l' := l'0); try easy.
-  rewrite mod_adder_half_sem with (B := B) 
-           (tenv := tenv) (tenv' := env'1)  (l := l) (l' := l'0); try easy.
+  lia. lia.
+  assert ((B + A) mod M < M) by (apply Nat.mod_upper_bound;lia).
+  simpl. lia.
+  rewrite mod_adder_half_sem with (B := B) (tenv := tenv); try easy.
   rewrite fbrev_twice_same. easy.
-  constructor. apply escope_rz_adder.
-  apply escope_rz_sub.
-  inv H20. constructor. easy. easy.
-  eapply typed_pexp_well_formed_ls.
-  apply H18. easy.
-  eapply typed_pexp_neu_prop.
-  apply H18. easy. easy.
+  apply well_typed_right_mode_pexp with (tenv := tenv); try easy.
+  apply mod_adder_half_well_typed; try easy.
+  apply qft_uniform_exp_trans with (tenv := tenv); try easy.
+  apply mod_adder_half_well_typed; try easy.
+  apply qft_gt_exp_trans with (tenv := tenv); try easy.
+  apply mod_adder_half_well_typed; try easy.
 Qed.
 
 Lemma phi_nor_mode_rz_modmult' : forall n size y x c aenv f A M, phi_modes f y size -> 
           nor_mode f c -> fst c <> y -> 0 < aenv y ->
-       nor_mode (prog_sem aenv (rz_modmult' y x n size c A M) f) c
-       /\ phi_modes (prog_sem aenv (rz_modmult' y x n size c A M) f) y size.
+       nor_mode (exp_sem aenv (rz_modmult' y x n size c A M) f) c
+       /\ phi_modes (exp_sem aenv (rz_modmult' y x n size c A M) f) y size.
 Proof.
   induction n; intros.
   simpl. split. easy. easy.
@@ -2201,7 +1816,7 @@ Proof.
  Local Transparent mod_adder.
  specialize (IHn size y x c aenv f A M H H0 H1 H2).
  destruct (get_cua
-      (prog_sem aenv (rz_modmult' y x n size c A M) f (x, size - S n))).
+      (exp_sem aenv (rz_modmult' y x n size c A M) f (x, size - S n))).
  split. apply nor_mode_mod_adder; try easy.
  apply phi_modes_mod_adder; try easy.
  apply IHn; try easy.
@@ -2251,61 +1866,60 @@ Qed.
 
 Lemma pexp_fresh_mod_adder : 
          forall m size x y c A M aenv, x <> y -> c <> (y,m) ->
-          pexp_fresh aenv (y,m) (mod_adder x size c A M).
+          exp_fresh aenv (y,m) (mod_adder x size c A M).
 Proof.
   unfold mod_adder. intros.
   constructor. constructor.
-  constructor. constructor. constructor.
+  constructor. constructor.
   apply exp_fresh_rz_adder'. easy.
   apply exp_fresh_rz_sub'. easy.
   constructor. constructor. constructor. unfold or_not_eq. left. iner_p.
   Local Transparent CNOT.
-  constructor. constructor. iner_p. constructor. destruct c. iner_p.
+  constructor. iner_p. constructor. destruct c. iner_p.
   Local Opaque CNOT.
   constructor. unfold or_not_eq. left. iner_p.
-  constructor. constructor. destruct c. iner_p.
+  constructor. destruct c. iner_p.
   apply exp_fresh_rz_adder'. easy.
   constructor. constructor.
-  constructor. apply exp_fresh_rz_sub'. easy.
+  apply exp_fresh_rz_sub'. easy.
   constructor. constructor. constructor. unfold or_not_eq. left. iner_p.
-  constructor. constructor. constructor. constructor. iner_p.
+  constructor. constructor. constructor. iner_p.
   Local Transparent CNOT.
   constructor. iner_p. constructor. destruct c. iner_p.
   Local Opaque CNOT.
   constructor. iner_p.
   constructor. unfold or_not_eq. left. iner_p.
-  constructor. apply fresh_inv_exp.
+  apply fresh_inv_exp.
   apply exp_fresh_rz_sub'. easy.
 Qed.
 
 Lemma pexp_fresh_mod_adder_ge : 
          forall m size x c A M aenv, fst c <> x -> aenv x = size -> 0 < size -> size <= m ->
-          pexp_fresh aenv (x,m) (mod_adder x size c A M).
+          exp_fresh aenv (x,m) (mod_adder x size c A M).
 Proof.
   unfold mod_adder. intros.
   constructor. constructor.
-  constructor. constructor. constructor.
+  constructor. constructor.
   apply exp_fresh_rz_adder'_ge; try lia.
   apply exp_fresh_rz_sub'_ge; try lia.
   constructor. constructor. constructor. unfold or_not_eq. right. rewrite H0. simpl. lia.
   Local Transparent CNOT.
-  constructor. constructor. iner_p. constructor. destruct c. iner_p.
+  constructor. iner_p. constructor. destruct c. iner_p.
   Local Opaque CNOT.
   constructor. unfold or_not_eq. right. rewrite H0. simpl. lia.
-  constructor. constructor. destruct c. iner_p.
+  constructor. destruct c. iner_p.
   apply exp_fresh_rz_adder'_ge; try lia.
   constructor. constructor.
-  constructor.
   apply exp_fresh_rz_sub'_ge; try lia.
   constructor. constructor.
   constructor. unfold or_not_eq. right. rewrite H0. simpl. lia.
-  constructor. constructor. constructor. constructor. iner_p.
+  constructor. constructor. constructor. iner_p.
   Local Transparent CNOT.
   constructor. iner_p. constructor. destruct c. iner_p.
   Local Opaque CNOT.
   constructor. iner_p.
   constructor. unfold or_not_eq. right. rewrite H0. simpl. lia.
-  constructor. apply fresh_inv_exp.
+  apply fresh_inv_exp.
   apply exp_fresh_rz_sub'_ge; try lia.
 Qed.
 
@@ -2346,10 +1960,10 @@ Opaque mod_adder.
 
 Lemma pexp_fresh_mod_mult: forall n m size x y c A M aenv, S n <= size -> m <= size - S n
              -> fst c <> x -> fst c <> y -> x <> y -> 
-            pexp_fresh aenv (x,m) (rz_modmult' y x n size c A M).
+            exp_fresh aenv (x,m) (rz_modmult' y x n size c A M).
 Proof.
   induction n;intros.
-  simpl. constructor. constructor. iner_p.
+  simpl. constructor. iner_p.
   simpl. constructor.
   apply IHn; try lia.
   constructor. iner_p.
@@ -2358,10 +1972,10 @@ Qed.
 
 Lemma pexp_fresh_mod_mult_real: forall n m size x y z c A M aenv, n <= size 
              -> c <> (z,m) -> z <> x -> z <> y -> 
-            pexp_fresh aenv (z,m) (rz_modmult' y x n size c A M).
+            exp_fresh aenv (z,m) (rz_modmult' y x n size c A M).
 Proof.
   induction n;intros.
-  simpl. constructor. constructor. iner_p.
+  simpl. constructor. iner_p.
   simpl. constructor.
   apply IHn; try lia. easy.
   constructor. iner_p.
@@ -2371,12 +1985,12 @@ Qed.
 
 Lemma rz_modmult'_x_same: forall n m size x y c A M aenv f, n <= size ->
             fst c <> x -> fst c <> y -> x <> y -> 
-             prog_sem aenv (rz_modmult' y x n size c A M) f (x,m) = f (x,m).
+             exp_sem aenv (rz_modmult' y x n size c A M) f (x,m) = f (x,m).
 Proof.
   induction n;intros. simpl. easy.
   simpl. 
-  destruct (get_cua (prog_sem aenv (rz_modmult' y x n size c A M) f (x, size - S n))).
-  rewrite fresh_pexp_sem_irrelevant.
+  destruct (get_cua (exp_sem aenv (rz_modmult' y x n size c A M) f (x, size - S n))).
+  rewrite efresh_exp_sem_irrelevant.
   rewrite IHn; try easy. lia.
   apply pexp_fresh_mod_adder; try easy. lia.
   destruct c. iner_p.
@@ -2385,12 +1999,12 @@ Qed.
 
 Lemma pexp_fresh_mod_mult_ge: forall n m size x y c A M aenv, 0 < n -> n <= size <= m -> aenv y = size
              -> fst c <> x -> fst c <> y -> x <> y -> 
-            pexp_fresh aenv (y,m) (rz_modmult' y x n size c A M).
+            exp_fresh aenv (y,m) (rz_modmult' y x n size c A M).
 Proof.
   induction n;intros.
-  simpl. constructor. constructor. iner_p.
+  simpl. constructor. iner_p.
   bdestruct (n =? 0). subst.
-  simpl. constructor. constructor. constructor. iner_p.
+  simpl. constructor. constructor. iner_p.
   constructor. iner_p.
   apply pexp_fresh_mod_adder_ge; try easy.
   simpl. constructor.
@@ -2398,337 +2012,296 @@ Proof.
   constructor. iner_p.
   apply pexp_fresh_mod_adder_ge; try easy. lia.
 Qed.
+
+Lemma exp_neu_rz_sub : forall n x y size M, n <= size -> exp_neu_l y [] (rz_sub' x n size M) [].
+Proof.
+ induction n;intros;simpl. constructor.
+ apply seq_neul with (l' := []).
+ apply IHn. lia.
+ destruct (M n). constructor. constructor.
+Qed.
+
+Lemma rz_modmult'_well_typed : forall n size x y c A M aenv tenv, n <= size ->
+          aenv y = size -> fst c <> x -> fst c <> y -> x <> y -> Env.MapsTo y (Phi (aenv y)) tenv
+               -> Env.MapsTo x Nor tenv -> Env.MapsTo (fst c) Nor tenv
+          -> well_typed_pexp aenv tenv (rz_modmult' y x n size c A M) tenv.
+Proof.
+ induction n; intros;simpl.
+ constructor. constructor.
+ apply pe_seq with (env' := tenv).
+ apply IHn; try easy. lia.
+ apply pcu_nor; try easy.
+ apply pexp_fresh_mod_adder; try easy. lia. destruct c. iner_p.
+ unfold exp_neu. intros.
+ Local Transparent mod_adder mod_adder_half CNOT.
+ unfold mod_adder,mod_adder_half.
+ apply seq_neul with (l' := []).
+ apply seq_neul with (l' := []).
+ apply seq_neul with (l' := []).
+ apply seq_neul with (l' := []).
+ apply exp_neu_rz_adder; try easy.
+ apply exp_neu_rz_sub; try easy.
+ apply seq_neul with (l' := []).
+ apply seq_neul with (l' := []).
+ constructor. apply cu_neul. constructor.
+ constructor. constructor.
+ apply exp_neu_rz_adder; try easy.
+ apply seq_neul with (l' := []).
+ apply seq_neul with (l' := []).
+ apply exp_neu_rz_sub; try easy.
+ apply seq_neul with (l' := []).
+ apply seq_neul with (l' := []).
+ constructor.
+ apply seq_neul with (l' := []).
+ apply seq_neul with (l' := []).
+ constructor.  constructor.  constructor.
+ constructor. constructor.
+ apply neu_l_inv_exp.
+ unfold exp_neu_prop. intros.
+ simpl in *.  lia.
+ apply exp_neu_rz_sub; try easy.
+ Local Opaque mod_adder mod_adder_half CNOT.
+ apply mod_adder_well_typed; try easy.
+Qed.
  
-Lemma rz_modmult'_typed_sem : forall n size y f x c A B M X aenv l l' tenv tenv', n <= S size ->
-         nor_modes f x (S size) -> phi_modes f y (S size) -> aenv y = S size ->
-          nor_mode f c -> fst c <> x -> fst c <> y -> x <> y -> get_cua (f c) = false
-        -> well_typed_pexp aenv l tenv (rz_modmult' y x n (S size) c A M) l' tenv'
-        -> right_mode_env aenv tenv f -> qft_uniform aenv tenv f -> qft_gt aenv tenv f
+Lemma rz_modmult'_typed_sem : forall n size y f x c A B M X aenv tenv, n <= S size ->
+          aenv y = S size -> fst c <> x -> fst c <> y -> x <> y -> 
+          Env.MapsTo y (Phi (aenv y)) tenv -> Env.MapsTo x Nor tenv -> Env.MapsTo (fst c) Nor tenv ->
+          get_cua (f c) = false -> snd c < aenv (fst c)
         -> 1 < M < 2^size -> A < M -> B < M -> X < 2^(S size) 
          -> fbrev (S size) (get_r_qft f y) = nat2fb B ->
-        fbrev (S size) (get_cus (S size) f x) = nat2fb X ->
-                  well_formed_ls l -> exp_neu_prop l ->
-            (prog_sem aenv (rz_modmult' y x n (S size) c A M) f c) = f c
-       /\ (get_r_qft (prog_sem aenv (rz_modmult' y x n (S size) c A M) f) y)
+        fbrev (S size) (get_cus (S size) f x) = nat2fb X
+        -> right_mode_env aenv tenv f -> qft_uniform aenv tenv f -> qft_gt aenv tenv f ->
+            (exp_sem aenv (rz_modmult' y x n (S size) c A M) f c) = f c
+       /\ (get_r_qft (exp_sem aenv (rz_modmult' y x n (S size) c A M) f) y)
            = (fbrev (S size) (nat2fb (((B + (bindecomp n X) * A) mod M)))).
 Proof.
   induction n; intros. simpl. split. easy.
  rewrite plus_0_r.
  rewrite Nat.mod_small by lia.
- rewrite <- H16.
+ rewrite <- H13.
  rewrite fbrev_twice_same. easy.
   Local Opaque mod_adder.
   simpl.
   Local Transparent mod_adder.
-  inv H8. inv H27.
  rewrite bindecomp_seq.
  rewrite mult_plus_distr_r.
- rewrite fresh_pexp_sem_irrelevant.
- assert ((get_cua (f (x, size - n))) = nat2fb X n).
+ rewrite efresh_exp_sem_irrelevant.
+ assert ((get_cua (f (@pair var nat x (size - n)))) = nat2fb X n).
  rewrite <- get_cus_cua with (n := (S size)) by lia.
- rewrite <- H17.
+ rewrite <- H14.
  unfold fbrev.
  bdestruct (n <? S size). simpl.
- assert ((size - 0 - n) = size - n) by lia. rewrite H20. easy. lia.
- destruct (get_cua (f (x, size - n))) eqn:eq1.
- rewrite mod_adder_sem with (B := (B + bindecomp n X * A) mod M)
-      (l := l') (l' := l') (tenv := tenv') (tenv' := tenv'); try easy.
- rewrite mod_adder_typed with (B := (B + bindecomp n X * A) mod M)
-      (l := l') (l' := l') (tenv := tenv') (tenv' := tenv'); try easy.
- rewrite <- H8. simpl.
+ assert ((size - 0 - n) = size - n) by lia. rewrite H19. easy. lia.
+ destruct (get_cua (f (@pair var nat x (size - n)))) eqn:eq1.
+ rewrite mod_adder_sem with (B := (B + bindecomp n X * A) mod M) (tenv := tenv); try easy.
+ rewrite mod_adder_typed with (B := (B + bindecomp n X * A) mod M) (tenv := tenv); try easy.
+ rewrite <- H18. simpl.
  rewrite <- Nat.add_mod by lia.
  rewrite plus_0_r.
  rewrite plus_assoc.
  split.
- specialize (IHn size y f x c A B M X aenv l l' tenv tenv').
+ specialize (IHn size y f x c A B M X aenv tenv).
  assert (n <= S size) by lia.
- specialize (IHn H20 H0 H1 H2 H3 H4 H5
-        H6 H7 H24 H9 H10 H11 H12 H13 H14 H15 H16 H17 H18 H19).
+ specialize (IHn H19 H0 H1 H2 H3 H4
+        H5 H6 H7 H8 H9 H10 H11 H12 H13 H14 H15 H16 H17).
  destruct IHn. 
- rewrite H23. easy. easy.
- apply phi_nor_mode_rz_modmult'; try easy. lia.
- apply phi_nor_mode_rz_modmult'; try easy. lia.
- specialize (IHn size y f x c A B M X aenv l l' tenv tenv').
+ rewrite H20. easy. easy. 
+ specialize (IHn size y f x c A B M X aenv tenv).
  assert (n <= S size) by lia.
- specialize (IHn H20 H0 H1 H2 H3 H4 H5
-        H6 H7 H24 H9 H10 H11 H12 H13 H14 H15 H16 H17 H18 H19).
+ specialize (IHn H19 H0 H1 H2 H3 H4
+        H5 H6 H7 H8 H9 H10 H11 H12 H13 H14 H15 H16 H17).
  destruct IHn. 
- rewrite H23. easy.
- apply well_typed_right_mode_pexp with (l := l) (l' := l') (tenv := tenv); try easy.
- apply qft_uniform_pexp_trans with (l := l) (l' := l') (tenv := tenv); try easy.
- apply qft_gt_pexp_trans with (l := l) (l' := l') (tenv := tenv); try easy.
+ rewrite H20. easy.
  apply Nat.mod_upper_bound ; lia.
  apply Nat.mod_upper_bound ; lia.
- specialize (IHn size y f x c A B M X aenv l l' tenv tenv').
+ specialize (IHn size y f x c A B M X aenv tenv).
  assert (n <= S size) by lia.
- specialize (IHn H20 H0 H1 H2 H3 H4 H5
-        H6 H7 H24 H9 H10 H11 H12 H13 H14 H15 H16 H17 H18 H19).
+ specialize (IHn H19 H0 H1 H2 H3 H4
+        H5 H6 H7 H8 H9 H10 H11 H12 H13 H14 H15 H16 H17).
  destruct IHn. 
- rewrite H25.
+ rewrite H21.
  rewrite fbrev_twice_same. easy.
- eapply typed_pexp_well_formed_ls. apply H24. easy.
- eapply typed_pexp_neu_prop. apply H24. easy. easy.
- apply phi_nor_mode_rz_modmult'; try easy. lia.
- apply phi_nor_mode_rz_modmult'; try easy. lia.
- specialize (IHn size y f x c A B M X aenv l l' tenv tenv').
+ apply well_typed_right_mode_pexp with (tenv := tenv); try easy.
+ apply rz_modmult'_well_typed; try easy. lia.
+ apply qft_uniform_exp_trans with (tenv := tenv); try easy.
+ apply rz_modmult'_well_typed; try easy. lia.
+ apply qft_gt_exp_trans with (tenv := tenv); try easy.
+ apply rz_modmult'_well_typed; try easy. lia.
+ specialize (IHn size y f x c A B M X aenv tenv).
  assert (n <= S size) by lia.
- specialize (IHn H20 H0 H1 H2 H3 H4 H5
-        H6 H7 H24 H9 H10 H11 H12 H13 H14 H15 H16 H17 H18 H19).
+ specialize (IHn H19 H0 H1 H2 H3 H4
+        H5 H6 H7 H8 H9 H10 H11 H12 H13 H14 H15 H16 H17).
  destruct IHn. 
- rewrite H23. easy.
- apply well_typed_right_mode_pexp with (l := l) (l' := l') (tenv := tenv); try easy.
- apply qft_uniform_pexp_trans with (l := l) (l' := l') (tenv := tenv); try easy.
- apply qft_gt_pexp_trans with (l := l) (l' := l') (tenv := tenv); try easy.
+ rewrite H20. easy.
  apply Nat.mod_upper_bound ; lia.
  apply Nat.mod_upper_bound ; lia.
- specialize (IHn size y f x c A B M X aenv l l' tenv tenv').
+ specialize (IHn size y f x c A B M X aenv tenv).
  assert (n <= S size) by lia.
- specialize (IHn H20 H0 H1 H2 H3 H4 H5
-        H6 H7 H24 H9 H10 H11 H12 H13 H14 H15 H16 H17 H18 H19).
+ specialize (IHn H19 H0 H1 H2 H3 H4
+        H5 H6 H7 H8 H9 H10 H11 H12 H13 H14 H15 H16 H17).
  destruct IHn. 
- rewrite H25.
+ rewrite H21.
  rewrite fbrev_twice_same. easy.
- eapply typed_pexp_well_formed_ls. apply H24. easy.
- eapply typed_pexp_neu_prop. apply H24. easy. easy.
- split.
- specialize (IHn size y f x c A B M X aenv l l' tenv tenv').
+ apply well_typed_right_mode_pexp with (tenv := tenv); try easy.
+ apply rz_modmult'_well_typed; try easy. lia.
+ apply qft_uniform_exp_trans with (tenv := tenv); try easy.
+ apply rz_modmult'_well_typed; try easy. lia.
+ apply qft_gt_exp_trans with (tenv := tenv); try easy.
+ apply rz_modmult'_well_typed; try easy. lia.
+ specialize (IHn size y f x c A B M X aenv tenv).
  assert (n <= S size) by lia.
- specialize (IHn H20 H0 H1 H2 H3 H4 H5
-        H6 H7 H24 H9 H10 H11 H12 H13 H14 H15 H16 H17 H18 H19).
- destruct IHn. 
- rewrite H23. easy.
- specialize (IHn size y f x c A B M X aenv l l' tenv tenv').
- assert (n <= S size) by lia.
- specialize (IHn H20 H0 H1 H2 H3 H4 H5
-        H6 H7 H24 H9 H10 H11 H12 H13 H14 H15 H16 H17 H18 H19).
- destruct IHn. 
- rewrite H25.
- rewrite <- H8. simpl.
+ specialize (IHn H19 H0 H1 H2 H3 H4
+        H5 H6 H7 H8 H9 H10 H11 H12 H13 H14 H15 H16 H17).
+ destruct IHn.
+ split. 
+ rewrite H20. easy.
+ rewrite H21.
+ rewrite <- H18. simpl.
  rewrite plus_0_r. easy.
- apply pexp_fresh_mod_mult; try lia.
+ apply pexp_fresh_mod_mult; try lia. easy. easy.
 Qed.
 
 Opaque rz_modmult'.
 
-Lemma nor_to_phi_modes: forall x size aenv f, aenv x >= size ->
-        nor_modes f x size -> phi_modes (prog_sem aenv (QFT x) f) x size.
-Proof.
-  intros.
-  unfold phi_modes, nor_modes in *.
-  intros.
-  simpl.
-  unfold turn_qft.
-  unfold phi_mode.
-  specialize (H0 i H1). unfold nor_mode in H0.
-  bdestruct (i <? aenv x).
-  rewrite assign_r_lt by lia.
-  unfold up_qft.
-  destruct (f (x,i)); try easy. lia.
-Qed.
-
-Lemma phi_to_nor_modes: forall x size aenv f, aenv x >= size ->
-        phi_modes f x size -> nor_modes (prog_sem aenv (RQFT x) f) x size.
-Proof.
-  intros.
-  unfold phi_modes, nor_modes in *.
-  intros.
-  simpl.
-  unfold turn_rqft.
-  unfold nor_mode.
-  specialize (H0 i H1). unfold nor_mode in H0.
-  bdestruct (i <? aenv x).
-  rewrite assign_seq_lt by lia. easy. lia.
-Qed.
-
-Lemma get_cus_qft_out : forall n x y f aenv,
-          x <> y -> (get_cus n (prog_sem aenv (QFT y) f) x) = get_cus n f x.
-Proof.
-  intros.
-  unfold get_cus.
-  apply functional_extensionality; intro.
-  bdestruct (x0 <? n).
-  rewrite fresh_pexp_sem_irrelevant. easy.
-  constructor. unfold or_not_eq. left. easy. easy.
-Qed.
-
-Lemma get_cus_assign_seq_aux : forall n i size x f g, i < n <= size ->
-      get_cus size (assign_seq f x g n) x i = g i.
-Proof.
-  induction n; intros; unfold get_cus in *; simpl.
-  lia.
-  specialize (IHn i size x f g).
-  bdestruct (i <? size).
-  bdestruct (i =? n). subst.
-  rewrite eupdate_index_eq. easy.
-  rewrite eupdate_index_neq by iner_p.
-  rewrite IHn. easy. lia.
-  lia.
-Qed.
-
-Lemma get_cus_assign_seq : forall size x f g,
-      (get_cus size (assign_seq f x g size) x) = cut_n g size.
-Proof.
-  intros.
-  apply functional_extensionality; intro.
-  unfold cut_n.
-  bdestruct (x0 <? size).
-  rewrite get_cus_assign_seq_aux.
-  easy. lia.
-  unfold get_cus.
-  bdestruct (x0 <? size). lia. easy.
-Qed.
-
-
-Lemma rz_modmult_half_typed : forall size y f x c A B M X aenv l l' tenv tenv',
-         nor_modes f x (S size) -> nor_modes f y (S size) -> aenv y = S size ->
-          nor_mode f c -> fst c <> x -> fst c <> y -> x <> y -> get_cua (f c) = false
-        -> well_typed_pexp aenv l tenv (rz_modmult_half y x (S size) c A M) l' tenv'
-        -> right_mode_env aenv tenv f -> qft_uniform aenv tenv f -> qft_gt aenv tenv f
+Lemma rz_modmult_half_typed : forall size y f x c A B M X aenv tenv,
+          aenv x = S size -> aenv y = S size -> fst c <> x -> fst c <> y -> x <> y -> 
+          Env.MapsTo y Nor tenv -> Env.MapsTo x Nor tenv -> Env.MapsTo (fst c) Nor tenv ->
+          get_cua (f c) = false -> snd c < aenv (fst c)
         -> 1 < M < 2^size -> A < M -> B < M -> X < 2^(S size) 
          -> fbrev (S size) (get_cus (S size) f y) = nat2fb B ->
-        fbrev (S size) (get_cus (S size) f x) = nat2fb X ->
-                  well_formed_ls l -> exp_neu_prop l ->
-            (prog_sem aenv (rz_modmult_half y x (S size) c A M) f c) = f c.
+        fbrev (S size) (get_cus (S size) f x) = nat2fb X
+        -> right_mode_env aenv tenv f -> qft_uniform aenv tenv f -> qft_gt aenv tenv f ->
+            (exp_sem aenv (rz_modmult_half y x (S size) c A M) f c) = f c.
 Proof.
   intros.
   assert (S size <= S size) by lia.
   unfold rz_modmult_half in *.
-  assert (prog_sem aenv ((QFT y;; rz_modmult' y x (S size) (S size) c A M);; RQFT y) f
-    = prog_sem aenv (RQFT y) 
-         (prog_sem aenv (rz_modmult' y x (S size) (S size) c A M)
-              (prog_sem aenv (QFT y) f))).
+  assert (exp_sem aenv ((QFT y; rz_modmult' y x (S size) (S size) c A M); RQFT y) f
+    = exp_sem aenv (RQFT y) 
+         (exp_sem aenv (rz_modmult' y x (S size) (S size) c A M)
+              (exp_sem aenv (QFT y) f))).
   simpl. easy.
-  rewrite H20. clear H20.
-  inv H7. inv H24. inv H27. inv H23.
-  specialize (rz_modmult'_typed_sem (S size) size y (prog_sem aenv (QFT y) f)
-          x c A B M X aenv l'1 l' env'0 env' H19) as eq1.
-  assert (nor_modes (prog_sem aenv (QFT y) f) x (S size)).
-  unfold nor_modes,nor_mode. intros.
-  rewrite fresh_pexp_sem_irrelevant. apply H; easy.
-  constructor. unfold or_not_eq. left. iner_p.
-  assert (phi_modes (prog_sem aenv (QFT y) f) y (S size)).
-  apply nor_to_phi_modes; try lia. easy.
-  assert (nor_mode (prog_sem aenv (QFT y) f) c).
-  unfold nor_mode.
-  rewrite fresh_pexp_sem_irrelevant. apply H2; easy.
-  constructor. unfold or_not_eq. left. iner_p.
-  assert (get_cua (prog_sem aenv (QFT y) f c) = false).
+  rewrite H19. clear H19.
+  specialize (rz_modmult'_typed_sem (S size) size y (exp_sem aenv (QFT y) f)
+          x c A B M X aenv (Env.add y (Phi (aenv y)) tenv) H18 H0 H1 H2 H3) as eq1.
+  assert (Env.MapsTo y (Phi (aenv y)) (Env.add y (Phi (aenv y)) tenv)).
+  apply Env.add_1. easy.
+  assert (Env.MapsTo x Nor (Env.add y (Phi (aenv y)) tenv)).
+  apply Env.add_2. lia. easy.
+  assert (Env.MapsTo (fst c) Nor (Env.add y (Phi (aenv y)) tenv)).
+  apply Env.add_2. lia. easy.
+  assert (get_cua (exp_sem aenv (QFT y) f c) = false).
   unfold get_cua.
-  rewrite fresh_pexp_sem_irrelevant.
-  destruct (f c); easy.
-  constructor. unfold or_not_eq. left. iner_p.
-  assert (right_mode_env aenv env'0 (prog_sem aenv (QFT y) f)).
-  apply well_typed_right_mode_pexp with 
-      (l := l'1) (l' := l'1) (tenv := tenv).
-  constructor; easy. easy.
-  assert (qft_uniform aenv env'0 (prog_sem aenv (QFT y) f)).
-  apply qft_uniform_pexp_trans with 
-      (l := l'1) (l' := l'1) (tenv := tenv). easy.
-  constructor; easy. easy.
-  assert (qft_gt aenv env'0 (prog_sem aenv (QFT y) f)).
-  apply qft_gt_pexp_trans with 
-      (l := l'1) (l' := l'1) (tenv := tenv). easy.
-  constructor; easy. easy.
-  assert (fbrev (S size) (get_r_qft (prog_sem aenv (QFT y) f) y) = nat2fb B).
+  rewrite efresh_exp_sem_irrelevant.
+  assert (nor_mode f c).
+  apply type_nor_mode with (aenv := aenv) (env := tenv); try easy.
+  unfold nor_mode in H22.
+  destruct (f c); easy. constructor. unfold or_not_eq. left. easy.
+  rewrite efresh_exp_sem_irrelevant.
+  assert (nor_modes f y (S size)).
+  rewrite <- H0.
+  apply type_nor_modes with (env := tenv); try easy.
+  assert (fbrev (S size) (get_r_qft (exp_sem aenv (QFT y) f) y) = nat2fb B).
   simpl.
   unfold turn_qft.
   unfold get_r_qft. rewrite assign_r_lt by lia.
   rewrite lshift_fun_0.
   unfold up_qft.
-  unfold nor_modes,nor_mode in H0.
+  unfold nor_modes,nor_mode in H23.
   assert (0 < S size) by lia.
-  specialize (H0 0 H31).
-  destruct (f (y, 0)); try easy.
-  rewrite H1. rewrite H15. easy.
-  assert (fbrev (S size) (get_cus (S size) (prog_sem aenv (QFT y) f) x) = nat2fb X).
+  specialize (H23 0 H24).
+  destruct (f (@pair var nat y O)); try easy.
+  rewrite H0. easy.
+  assert (fbrev (S size) (get_cus (S size) (exp_sem aenv (QFT y) f) x) = nat2fb X).
   rewrite get_cus_qft_out. easy. easy.
-  specialize (eq1 H7 H22 H1 H23 H3 H4 H5 H25 
-            H28 H27 H29 H30 H11 H12 H13 H14 H31 H32 H17 H18).
+  assert (right_mode_env aenv (Env.add y (Phi (aenv y)) tenv)
+        (exp_sem aenv (QFT y) f) ).
+  apply well_typed_right_mode_pexp with (tenv := tenv); try easy.
+  apply qft_nor. easy. easy.
+  assert (qft_uniform aenv (Env.add y (Phi (aenv y)) tenv) (exp_sem aenv (QFT y) f)).
+  apply qft_uniform_exp_trans with (tenv := tenv); try easy.
+  apply qft_nor. easy. easy.
+  assert (qft_gt aenv (Env.add y (Phi (aenv y)) tenv) (exp_sem aenv (QFT y) f)).
+  apply qft_gt_exp_trans with (tenv := tenv); try easy.
+  apply qft_nor. easy. easy.
+  specialize (eq1 H19 H20 H21 H22 H8 H9 H10 H11 H12 H24 H25 H26 H27 H28).
   destruct eq1.
-  remember ((prog_sem aenv (rz_modmult' y x 
-         (S size) (S size) c A M) (prog_sem aenv (QFT y) f))) as g.
-  simpl.
-  unfold turn_rqft.
-  rewrite assign_seq_out by lia.
-  subst.
-  rewrite H33. simpl.
-  unfold turn_qft.
-  rewrite assign_r_out by lia. easy.
+  rewrite H29.
+  rewrite efresh_exp_sem_irrelevant. easy.
+  constructor. unfold or_not_eq. left. easy.
+  constructor. unfold or_not_eq. left. easy.
 Qed.
 
-Lemma rz_modmult_half_sem : forall size y f x c A B M X aenv l l' tenv tenv',
-         nor_modes f x (S size) -> nor_modes f y (S size) -> aenv y = S size ->
-          nor_mode f c -> fst c <> x -> fst c <> y -> x <> y -> get_cua (f c) = false
-        -> well_typed_pexp aenv l tenv (rz_modmult_half y x (S size) c A M) l' tenv'
-        -> right_mode_env aenv tenv f -> qft_uniform aenv tenv f -> qft_gt aenv tenv f
+Lemma rz_modmult_half_sem : forall size y f x c A B M X aenv tenv,
+          aenv x = S size -> aenv y = S size -> fst c <> x -> fst c <> y -> x <> y -> 
+          Env.MapsTo y Nor tenv -> Env.MapsTo x Nor tenv -> Env.MapsTo (fst c) Nor tenv ->
+          get_cua (f c) = false -> snd c < aenv (fst c)
         -> 1 < M < 2^size -> A < M -> B < M -> X < 2^(S size) 
          -> fbrev (S size) (get_cus (S size) f y) = nat2fb B ->
-        fbrev (S size) (get_cus (S size) f x) = nat2fb X ->
-                  well_formed_ls l -> exp_neu_prop l ->
-            get_cus (S size) (prog_sem aenv (rz_modmult_half y x (S size) c A M) f) y
+        fbrev (S size) (get_cus (S size) f x) = nat2fb X
+        -> right_mode_env aenv tenv f -> qft_uniform aenv tenv f -> qft_gt aenv tenv f ->
+            get_cus (S size) (exp_sem aenv (rz_modmult_half y x (S size) c A M) f) y
                    = (fbrev (S size) (nat2fb (((B + X * A) mod M)))).
 Proof.
   intros.
   assert (S size <= S size) by lia.
   unfold rz_modmult_half in *.
-  assert (prog_sem aenv ((QFT y;; rz_modmult' y x (S size) (S size) c A M);; RQFT y) f
-    = prog_sem aenv (RQFT y) 
-         (prog_sem aenv (rz_modmult' y x (S size) (S size) c A M)
-              (prog_sem aenv (QFT y) f))).
+  assert (exp_sem aenv ((QFT y; rz_modmult' y x (S size) (S size) c A M); RQFT y) f
+    = exp_sem aenv (RQFT y) 
+         (exp_sem aenv (rz_modmult' y x (S size) (S size) c A M)
+              (exp_sem aenv (QFT y) f))).
   simpl. easy.
-  rewrite H20. clear H20.
-  inv H7. inv H24. inv H27. inv H23.
-  specialize (rz_modmult'_typed_sem (S size) size y (prog_sem aenv (QFT y) f)
-          x c A B M X aenv l'1 l' env'0 env' H19) as eq1.
-  assert (nor_modes (prog_sem aenv (QFT y) f) x (S size)).
-  unfold nor_modes,nor_mode. intros.
-  rewrite fresh_pexp_sem_irrelevant. apply H; easy.
-  constructor. unfold or_not_eq. left. iner_p.
-  assert (phi_modes (prog_sem aenv (QFT y) f) y (S size)).
-  apply nor_to_phi_modes; try lia. easy.
-  assert (nor_mode (prog_sem aenv (QFT y) f) c).
-  unfold nor_mode.
-  rewrite fresh_pexp_sem_irrelevant. apply H2; easy.
-  constructor. unfold or_not_eq. left. iner_p.
-  assert (get_cua (prog_sem aenv (QFT y) f c) = false).
+  rewrite H19. clear H19.
+  specialize (rz_modmult'_typed_sem (S size) size y (exp_sem aenv (QFT y) f)
+          x c A B M X aenv (Env.add y (Phi (aenv y)) tenv) H18 H0 H1 H2 H3) as eq1.
+  assert (Env.MapsTo y (Phi (aenv y)) (Env.add y (Phi (aenv y)) tenv)).
+  apply Env.add_1. easy.
+  assert (Env.MapsTo x Nor (Env.add y (Phi (aenv y)) tenv)).
+  apply Env.add_2. lia. easy.
+  assert (Env.MapsTo (fst c) Nor (Env.add y (Phi (aenv y)) tenv)).
+  apply Env.add_2. lia. easy.
+  assert (get_cua (exp_sem aenv (QFT y) f c) = false).
   unfold get_cua.
-  rewrite fresh_pexp_sem_irrelevant.
-  destruct (f c); easy.
-  constructor. unfold or_not_eq. left. iner_p.
-  assert (right_mode_env aenv env'0 (prog_sem aenv (QFT y) f)).
-  apply well_typed_right_mode_pexp with 
-      (l := l'1) (l' := l'1) (tenv := tenv).
-  constructor; easy. easy.
-  assert (qft_uniform aenv env'0 (prog_sem aenv (QFT y) f)).
-  apply qft_uniform_pexp_trans with 
-      (l := l'1) (l' := l'1) (tenv := tenv). easy.
-  constructor; easy. easy.
-  assert (qft_gt aenv env'0 (prog_sem aenv (QFT y) f)).
-  apply qft_gt_pexp_trans with 
-      (l := l'1) (l' := l'1) (tenv := tenv). easy.
-  constructor; easy. easy.
-  assert (fbrev (S size) (get_r_qft (prog_sem aenv (QFT y) f) y) = nat2fb B).
+  rewrite efresh_exp_sem_irrelevant.
+  assert (nor_mode f c).
+  apply type_nor_mode with (aenv := aenv) (env := tenv); try easy.
+  unfold nor_mode in H22.
+  destruct (f c); easy. constructor. unfold or_not_eq. left. easy.
+  assert (nor_modes f y (S size)).
+  rewrite <- H0.
+  apply type_nor_modes with (env := tenv); try easy.
+  assert (fbrev (S size) (get_r_qft (exp_sem aenv (QFT y) f) y) = nat2fb B).
   simpl.
   unfold turn_qft.
   unfold get_r_qft. rewrite assign_r_lt by lia.
   rewrite lshift_fun_0.
   unfold up_qft.
-  unfold nor_modes,nor_mode in H0.
+  unfold nor_modes,nor_mode in H23.
   assert (0 < S size) by lia.
-  specialize (H0 0 H31).
-  destruct (f (y, 0)); try easy.
-  rewrite H1. rewrite H15. easy.
-  assert (fbrev (S size) (get_cus (S size) (prog_sem aenv (QFT y) f) x) = nat2fb X).
+  specialize (H23 0 H24).
+  destruct (f (@pair var nat y O)); try easy.
+  rewrite H0. easy.
+  assert (fbrev (S size) (get_cus (S size) (exp_sem aenv (QFT y) f) x) = nat2fb X).
   rewrite get_cus_qft_out. easy. easy.
-  specialize (eq1 H7 H22 H1 H23 H3 H4 H5 H25 
-            H28 H27 H29 H30 H11 H12 H13 H14 H31 H32 H17 H18).
+  assert (right_mode_env aenv (Env.add y (Phi (aenv y)) tenv)
+        (exp_sem aenv (QFT y) f) ).
+  apply well_typed_right_mode_pexp with (tenv := tenv); try easy.
+  apply qft_nor. easy. easy.
+  assert (qft_uniform aenv (Env.add y (Phi (aenv y)) tenv) (exp_sem aenv (QFT y) f)).
+  apply qft_uniform_exp_trans with (tenv := tenv); try easy.
+  apply qft_nor. easy. easy.
+  assert (qft_gt aenv (Env.add y (Phi (aenv y)) tenv) (exp_sem aenv (QFT y) f)).
+  apply qft_gt_exp_trans with (tenv := tenv); try easy.
+  apply qft_nor. easy. easy.
+  specialize (eq1 H19 H20 H21 H22 H8 H9 H10 H11 H12 H24 H25 H26 H27 H28).
   destruct eq1.
-  remember ((prog_sem aenv (rz_modmult' y x 
-         (S size) (S size) c A M) (prog_sem aenv (QFT y) f))) as g.
+  remember ((exp_sem aenv (rz_modmult' y x 
+         (S size) (S size) c A M) (exp_sem aenv (QFT y) f))) as g.
   simpl.
-  unfold turn_rqft. rewrite H1.
+  unfold turn_rqft. rewrite H0.
   rewrite get_cus_assign_seq.
-  rewrite H34.
+  rewrite H30.
   rewrite cut_n_fbrev_flip.
   rewrite cut_n_mod.
   rewrite bindecomp_spec.
@@ -2740,7 +2313,7 @@ Qed.
 
 Lemma rz_modmult_half_x_same: forall size y c A M aenv f x m,
             fst c <> x -> fst c <> y -> x <> y -> 
-             prog_sem aenv (rz_modmult_half y x size c A M) f (x,m) = f (x,m).
+             exp_sem aenv (rz_modmult_half y x size c A M) f (x,m) = f (x,m).
 Proof.
   intros. unfold rz_modmult_half. simpl.
   unfold turn_rqft.
@@ -2753,7 +2326,7 @@ Qed.
 Lemma rz_modmult_half_r : forall i size y f x c A M aenv, i < size ->
          nor_modes f x (size) -> nor_modes f y (size) -> aenv y = size ->
           nor_mode f c -> fst c <> x -> fst c <> y -> x <> y ->
-            get_r ((prog_sem aenv 
+            get_r ((exp_sem aenv 
                  (rz_modmult_half y x (size) c A M) f) (y,i)) = get_r (f (y,i)).
 Proof.
   intros.
@@ -2765,7 +2338,7 @@ Admitted.
 
 Lemma rz_modmult_half_x_cus: forall size y c A M aenv f x,
             fst c <> x -> fst c <> y -> x <> y -> 
-          get_cus size (prog_sem aenv 
+          get_cus size (exp_sem aenv 
              (rz_modmult_half y x size c A M) f) x = get_cus size f x.
 Proof.
   intros. unfold get_cus.
@@ -2774,27 +2347,32 @@ Proof.
   rewrite rz_modmult_half_x_same; try easy. easy.
 Qed.
 
-Lemma rz_modmult_half_sem_1 : forall size y f x c A B M X aenv l l' tenv tenv',
-         nor_modes f x (S size) -> nor_modes f y (S size) -> aenv y = S size ->
-          nor_mode f c -> fst c <> x -> fst c <> y -> x <> y -> get_cua (f c) = false
-        -> well_typed_pexp aenv l tenv (rz_modmult_half y x (S size) c A M) l' tenv'
-        -> right_mode_env aenv tenv f -> qft_uniform aenv tenv f -> qft_gt aenv tenv f
+Lemma rz_modmult_half_sem_1 : forall size y f x c A B M X aenv tenv,
+          aenv x = S size -> aenv y = S size -> fst c <> x -> fst c <> y -> x <> y -> 
+          Env.MapsTo y Nor tenv -> Env.MapsTo x Nor tenv -> Env.MapsTo (fst c) Nor tenv ->
+          get_cua (f c) = false -> snd c < aenv (fst c)
         -> 1 < M < 2^size -> A < M -> B < M -> X < 2^(S size) 
          -> fbrev (S size) (get_cus (S size) f y) = nat2fb B ->
-        fbrev (S size) (get_cus (S size) f x) = nat2fb X ->
-                  well_formed_ls l -> exp_neu_prop l ->
-           (prog_sem aenv (rz_modmult_half y x (S size) c A M) f)
+        fbrev (S size) (get_cus (S size) f x) = nat2fb X
+        -> right_mode_env aenv tenv f -> qft_uniform aenv tenv f -> qft_gt aenv tenv f ->
+           (exp_sem aenv (rz_modmult_half y x (S size) c A M) f)
                    = put_cus f y (fbrev (S size) (nat2fb (((B + X * A) mod M)))) (S size).
 Proof.
   intros.
-  rewrite <- (rz_modmult_half_sem size y f x c A B M X aenv l l' tenv tenv'); try easy.
+  rewrite <- (rz_modmult_half_sem size y f x c A B M X aenv tenv); try easy.
   apply functional_extensionality; intros.
   destruct x0.
   bdestruct (v =? y). subst.
   bdestruct (n <? S size). 
   rewrite put_cus_eq by lia.
   rewrite get_cus_cua by lia.
-  assert (nor_modes (prog_sem aenv (rz_modmult_half y x (S size) c A M) f) y (S size)).
+  assert (nor_modes f y (S size)) as X1.
+  rewrite <- H0.
+  apply type_nor_modes with (env := tenv); try easy.
+  assert (nor_modes f x (S size)) as X2.
+  rewrite <- H.
+  apply type_nor_modes with (env := tenv); try easy.
+  assert (nor_modes (exp_sem aenv (rz_modmult_half y x (S size) c A M) f) y (S size)).
   unfold rz_modmult_half.
   simpl.
   unfold turn_rqft.
@@ -2803,30 +2381,29 @@ Proof.
   unfold nor_mode.
   rewrite assign_seq_lt;try lia.
   unfold nor_modes,nor_mode in H1.
-  specialize (H0 n H19) as eq1. unfold nor_mode in eq1.
+  specialize (X1 n H18) as eq1. unfold nor_mode in eq1.
   unfold put_cu.
-  destruct (f (y,n)) eqn:eq2.
-  assert (get_r (prog_sem aenv (rz_modmult_half y x (S size) c A M) f (y, n)) = r).
+  destruct (f (@pair var nat y n)) eqn:eq2.
+  assert (get_r (exp_sem aenv (rz_modmult_half y x (S size) c A M) f (@pair var nat y n)) = r).
   rewrite rz_modmult_half_r; try easy. rewrite eq2. unfold get_r. easy.
-  unfold nor_modes in H20.
-  specialize (H20 n H19). unfold nor_mode in H20.
-  destruct (prog_sem aenv (rz_modmult_half y x (S size) c A M) f (y, n)).
-  unfold get_cua. unfold get_r in H21. subst. easy. 
-  lia. lia. lia. lia.
+  apply type_nor_mode with (aenv:=aenv) (env := tenv); try easy.
+  unfold nor_modes in H19.
+  specialize (H19 n H18). unfold nor_mode in H19.
+  destruct (exp_sem aenv (rz_modmult_half y x (S size) c A M) f (@pair var nat y n)).
+  unfold get_cua. unfold get_r in H20. subst. easy. lia. lia. lia. lia.
   rewrite put_cus_neq_2; try lia.
-  rewrite fresh_pexp_sem_irrelevant; try easy.
+  rewrite efresh_exp_sem_irrelevant; try easy.
   unfold rz_modmult_half.
   constructor. constructor.
-  constructor. unfold or_not_eq. right. rewrite H1. simpl. lia.
-  apply pexp_fresh_mod_mult_ge; try lia.
-  constructor. unfold or_not_eq. right. rewrite H1. simpl. lia.
+  constructor. unfold or_not_eq. right. rewrite H0. simpl. lia.
+  apply pexp_fresh_mod_mult_ge; try lia. easy. easy.
+  constructor. unfold or_not_eq. right. rewrite H0. simpl. lia.
   rewrite put_cus_neq; try lia.
   bdestruct (v =? x). subst.
-  rewrite rz_modmult_half_x_same; try lia. easy.
+  rewrite rz_modmult_half_x_same; try lia. easy. easy. easy.
   bdestruct (c ==? (v,n)). subst.
-  rewrite rz_modmult_half_typed with (B := B) (X := X)
-           (l:=l) (l':=l') (tenv:=tenv) (tenv':=tenv'); try easy.
-  rewrite fresh_pexp_sem_irrelevant; try easy.
+  rewrite rz_modmult_half_typed with (B := B) (X := X) (tenv:=tenv); try easy.
+  rewrite efresh_exp_sem_irrelevant; try easy.
   unfold rz_modmult_half.
   constructor. constructor.
   constructor. unfold or_not_eq. left. simpl. easy.
@@ -2836,86 +2413,78 @@ Qed.
 
 Opaque rz_modmult_half.
 
-Lemma rz_modmult_full_sem : forall size y f x c A Ainv M X aenv l tenv ,
-         nor_modes f x (S size) -> nor_modes f y (S size) -> aenv y = S size -> aenv x = S size ->
-          nor_mode f c -> fst c <> x -> fst c <> y -> x <> y -> get_cua (f c) = false
-        -> well_typed_pexp aenv l tenv (rz_modmult_full y x (S size) c A Ainv M) l tenv
-        -> right_mode_env aenv tenv f -> qft_uniform aenv tenv f -> qft_gt aenv tenv f
+Lemma rz_modmult_full_sem : forall size y f x c A Ainv M X aenv tenv ,
+          aenv x = S size -> aenv y = S size -> fst c <> x -> fst c <> y -> x <> y -> 
+          Env.MapsTo y Nor tenv -> Env.MapsTo x Nor tenv -> Env.MapsTo (fst c) Nor tenv ->
+          get_cua (f c) = false -> snd c < aenv (fst c)
         -> 1 < M < 2^size -> A < M -> Ainv < M -> X < M -> A * Ainv mod M = 1
          -> fbrev (S size) (get_cus (S size) f y) = nat2fb 0 ->
-            fbrev (S size) (get_cus (S size) f x) = nat2fb X ->
-                  well_formed_ls l -> exp_neu_prop l ->
-            (prog_sem aenv (rz_modmult_full y x (S size) c A Ainv M) f)
+            fbrev (S size) (get_cus (S size) f x) = nat2fb X
+        -> right_mode_env aenv tenv f -> qft_uniform aenv tenv f -> qft_gt aenv tenv f ->
+            (exp_sem aenv (rz_modmult_full y x (S size) c A Ainv M) f)
                    = put_cus (put_cus f y (fbrev (S size) (nat2fb (((X * A) mod M)))) (S size)) 
                                     x (fbrev (S size) (nat2fb 0)) (S size).
 Proof.
   intros. simpl.
-  inv H8.
-  apply inv_pexp_reverse with (l := l) 
-       (l' := l') (tenv := tenv) (tenv' := env'); try easy.
-  assert (rz_modmult_half x y (S size) c Ainv M 
-            = inv_pexp (inv_pexp (rz_modmult_half x y (S size) c Ainv M))).
-  rewrite inv_pexp_involutive. easy.
-  rewrite H8. clear H8.
-  apply typed_inv_pexp.
-  eapply typed_pexp_well_formed_ls. apply H25. easy.
-  eapply typed_pexp_neu_prop. apply H25. easy. easy. easy.
+  assert (nor_modes f y (S size)) as X1.
+  rewrite <- H0. apply type_nor_modes with (env := tenv). easy. easy.
+  assert (nor_modes f x (S size)) as X2.
+  rewrite <- H. apply type_nor_modes with (env := tenv). easy. easy.
+  apply inv_pexp_reverse with (tenv := tenv) (tenv' := tenv); try easy.
+  Local Transparent rz_modmult_half.
+  unfold rz_modmult_half.
+  apply pe_seq with (env' := Env.add x (Phi (aenv x)) tenv). 
+  apply pe_seq with (env' := Env.add x (Phi (aenv x)) tenv). 
+  apply qft_nor. easy. easy.
+  apply rz_modmult'_well_typed; try easy. lia.
+  apply Env.add_1. easy.
+  apply Env.add_2. lia. easy.
+  apply Env.add_2. iner_p. easy.
+  apply rqft_phi.
+  apply Env.add_1. easy.
+ apply EnvFacts.Equal_mapsto_iff.
+ intros. split. intros.
+ bdestruct (k =? x). subst.
+ apply mapsto_always_same with (v2 := e) in H5. subst.
+ apply Env.add_1. easy. easy.
+ apply Env.add_2. lia. apply Env.add_2. lia. easy.
+ intros.
+ bdestruct (k =? x). subst. 
+ apply mapsto_add1 in H19. subst. easy.
+ apply Env.add_3 in H19. apply Env.add_3 in H19. easy. lia. lia.
+  Local Opaque rz_modmult_half.
   apply right_mode_exp_put_cus_same.
   apply right_mode_exp_put_cus_same. easy.
   apply qft_uniform_put_cus_same.
   apply qft_uniform_put_cus_same. easy. easy.
   apply right_mode_exp_put_cus_same. easy.
   apply qft_gt_put_cus_same.
-  apply qft_gt_put_cus_same. easy. easy.
+  apply qft_gt_put_cus_same. easy.
+  easy.
   unfold nor_modes in *. intros.
-  nor_mode_simpl. apply H; lia.
-  rewrite rz_modmult_half_sem_1 with (y := y) (x:= x) (l := l) (tenv:=tenv)
-           (l':=l') (tenv':=env') (B:=0) (X := X); try easy.
-  assert (well_typed_pexp 
-           aenv l tenv (rz_modmult_half x y (S size) c Ainv M) l' env').
-  assert (rz_modmult_half x y (S size) c Ainv M 
-            = inv_pexp (inv_pexp (rz_modmult_half x y (S size) c Ainv M))).
-  rewrite inv_pexp_involutive. easy.
-  rewrite H8.
-  apply typed_inv_pexp.
-  eapply typed_pexp_well_formed_ls. apply H25. easy.
-  eapply typed_pexp_neu_prop. apply H25. easy. easy. easy.
-  rewrite plus_0_l.
-  rewrite rz_modmult_half_sem_1 with (y := x) (x:= y) (l := l) (tenv:=tenv)
-           (l':=l') (tenv':=env') (B:=0) (X := ((X * A) mod M)); try easy.
+  nor_mode_simpl. apply X2; lia.
+  rewrite rz_modmult_half_sem_1 with (y := y) (x:= x) (tenv:=tenv) (B:=0) (X := X); try easy.
+  rewrite rz_modmult_half_sem_1 with (y := x) (x:= y) (tenv:=tenv) (B:=0) (X := ((X * A) mod M)).
   rewrite put_cus_twice_eq.
+  rewrite plus_0_l.
   rewrite plus_0_l.
   rewrite Nat.mul_mod_idemp_l by lia.
   rewrite <- Nat.mul_assoc.
   rewrite (Nat.mul_mod X (A * Ainv)) by lia.
-  rewrite H16.
+  rewrite H13.
   rewrite Nat.mul_1_r.
   rewrite Nat.mod_mod by lia.
   rewrite (Nat.mod_small X) by easy.
   apply put_cus_same.
   unfold nor_modes; intros.
-  nor_mode_simpl. apply H. easy.
+  nor_mode_simpl. apply X2. easy.
   rewrite get_cus_put_neq by lia.
-  rewrite <- H18.
+  rewrite <- H15.
   rewrite fbrev_twice_same. easy.
-  unfold nor_modes; intros.
-  nor_mode_simpl. apply H0. easy.
-  unfold nor_modes; intros.
-  nor_mode_simpl. apply H. easy.
-  destruct c.
-  nor_mode_simpl. lia.
+  1-4:easy. lia. 1-3:easy.
   destruct c.
   rewrite cus_get_neq by iner_p.
-  rewrite cus_get_neq by iner_p. easy.
-  apply right_mode_exp_put_cus_same.
-  apply right_mode_exp_put_cus_same. easy.
-  apply qft_uniform_put_cus_same.
-  apply qft_uniform_put_cus_same. easy. easy.
-  apply right_mode_exp_put_cus_same. easy.
-  apply qft_gt_put_cus_same.
-  apply qft_gt_put_cus_same. easy. easy.
-  unfold nor_modes; intros.
-  nor_mode_simpl. apply H. easy. lia.
+  rewrite cus_get_neq by iner_p. easy. 1-3:easy. lia.
   assert ((X * A) mod M < M).
   apply Nat.mod_upper_bound. lia. simpl. lia.
   rewrite put_cus_twice_neq by lia.
@@ -2933,10 +2502,16 @@ Proof.
   rewrite Nat.mod_small. easy. 
   assert ((X * A) mod M < M).
   apply Nat.mod_upper_bound. lia. simpl. lia.
-  lia. simpl. lia.
+  apply right_mode_exp_put_cus_same.
+  apply right_mode_exp_put_cus_same. easy.
+  apply qft_uniform_put_cus_same.
+  apply qft_uniform_put_cus_same. easy. easy.
+  apply right_mode_exp_put_cus_same. easy.
+  apply qft_gt_put_cus_same.
+  apply qft_gt_put_cus_same. easy. easy.
+  unfold nor_modes; intros.
+  nor_mode_simpl. apply X2. easy. lia. simpl. lia.
 Qed.
-
-
 
 (** Functions for extraction & evaluation: **)
 (* Implementing x * M multiplier. *)
@@ -2947,8 +2522,8 @@ Fixpoint nat_mult' (n:nat) (size:nat) (x:var) (ex:var) (M:nat->bool) :=
           nat_mult' m size x ex (cut_n (times_two_spec M) size)
   end.
 Definition nat_mult (size:nat) (x:var) (re:var) (M:nat -> bool) := 
-  Exp (Rev x; Rev re) ;; QFT re ;; nat_mult' size size x re M;; 
-  RQFT re;; inv_pexp (Exp (Rev x; Rev re)).
+   (Rev x; Rev re) ; QFT re ; nat_mult' size size x re M;
+  RQFT re; inv_exp ( (Rev x; Rev re)).
 
 Definition vars_for_rz_nat_m (size:nat) := gen_vars size (x_var::y_var::[]).
 
@@ -2963,7 +2538,7 @@ Fixpoint flt_mult' (n:nat) (size:nat) (x:var) (ex:var) (M:nat->bool) :=
           flt_mult' m size x ex (cut_n (div_two_spec M) size)
   end.
 Definition flt_mult (size:nat) (x re:var) (M:nat -> bool) := 
-  Exp (Rev x; Rev re) ;; flt_mult' size size x re M;; inv_pexp (Exp (Rev x; Rev re)).
+   (Rev x; Rev re) ; flt_mult' size size x re M; inv_exp ( (Rev x; Rev re)).
 
 (* Implementing x * y multiplier for nats values. *)
 (* y is in nor_mode, and y is in phi, [y][x] -> [y][x+y] *)
@@ -2987,9 +2562,9 @@ Fixpoint nat_full_mult' (n:nat) (size:nat) (x:var) (y:var) (re:var) :=
    [x][y][phi(re)] ->[x][y][phi(x*y mod 2^n)], re is supposed to be zero, 
    ex is in nor_mode. *)
 Definition nat_full_mult (size:nat) (x y:var) (re:var) :=
-  Exp (Rev re ; Rev x);; QFT re ;;
-  Exp (nat_full_mult' size size x y re) ;;
-  RQFT re ;; Exp (Rev re; Rev x).
+   (Rev re ; Rev x); QFT re ;
+   (nat_full_mult' size size x y re) ;
+  RQFT re ;  (Rev re; Rev x).
 
 Definition vars_for_rz_nat_full_m (size:nat) := 
   gen_vars size (x_var::y_var::z_var::[]).
@@ -3025,9 +2600,9 @@ Fixpoint clean_high_flt (n:nat) (size:nat) (y:var) (ex:var) :=
    [x][y][phi(re)] ->[x][y][phi((x*2^n*y)/2^n)], re is supposed to be zero, 
    ex is in nor_mode. *)
 Definition flt_full_mult (size:nat) (x y:var) (re:var) (ex:var) :=
-  Exp (Rev re; Rev x; Rev y);; QFT re ;;
-  Exp (flt_full_mult_quar size x y re ex ; inv_exp (clean_high_flt size size y ex)) ;;
-  RQFT re ;;(Exp (Rev re; Rev x; Rev y)).
+   (Rev re; Rev x; Rev y); QFT re ;
+   (flt_full_mult_quar size x y re ex ; inv_exp (clean_high_flt size size y ex)) ;
+  RQFT re ;( (Rev re; Rev x; Rev y)).
 
 (*
 Definition moddoubler01 n x M c1 c2 :=
@@ -3043,18 +2618,18 @@ Fixpoint modsummer' i n M x y c1 c2 s (fC : nat -> bool) :=
 
 (* Implementing x < M comparator. *)
 Definition rz_comparator (x:var) (n:nat) (c:posi) (M:nat) := 
-  Exp (Rev x);; QFT x;; Exp (rz_sub x n (nat2fb M));; RQFT x ;; Exp (CNOT (x,0) c);; 
-  inv_pexp (Exp (Rev x);; QFT x;; Exp (rz_sub x n (nat2fb M));; RQFT x).
+   (Rev x); QFT x;  (rz_sub x n (nat2fb M)); RQFT x ; (CNOT (x,0) c);
+  inv_exp ( (Rev x); QFT x; (rz_sub x n (nat2fb M)); RQFT x).
 
 
 (* Implementing x + y / X + M addition. *)
 Definition rz_full_adder_form (x:var) (n:nat) (y:var) :=
-  Exp (Rev x; Rev y);; QFT x ;; rz_full_adder x n y ;; 
-  inv_pexp (Exp (Rev x; Rev y);; QFT x).
+   (Rev x; Rev y); QFT x ; rz_full_adder x n y ; 
+  inv_exp ( (Rev x; Rev y); QFT x).
 
 Definition rz_adder_form (x:var) (n:nat) (M:nat -> bool) :=
-  Exp (Rev x);; QFT x;; rz_adder x n M ;; 
-  inv_pexp (Exp (Rev x);; QFT x).
+   (Rev x); QFT x; rz_adder x n M ;
+  inv_exp ( (Rev x); QFT x).
 
 Definition vars_for_rz_adder (size:nat) := gen_vars size (x_var::[]).
 
@@ -3072,47 +2647,47 @@ Fixpoint rz_full_sub (x:var) (n:nat) (y:var) :=
   end.
 
 Definition rz_full_sub_form (x:var) (n:nat) (y:var) :=
-  Exp (Rev x; Rev y);; QFT x ;; rz_full_sub x n y ;; 
-  inv_pexp (Exp (Rev x; Rev y);; QFT x).
+   (Rev x; Rev y); QFT x ; rz_full_sub x n y ; 
+  inv_exp ( (Rev x; Rev y); QFT x).
 
 (* Implementing x - M subtractor. *)
 Definition rz_sub_right (x:var) (n:nat) (M:nat -> bool) :=
-  Exp (Rev x);; QFT x;; rz_sub x n M ;; inv_pexp (Exp (Rev x);; QFT x).
+   (Rev x); QFT x; rz_sub x n M ; inv_exp ( (Rev x); QFT x).
 
 (* Implementing M - x subtractor. *)
 Definition rz_sub_left (M:nat -> bool) (x:var) (n:nat) :=
-  Exp (Rev x);; QFT x;; rz_sub x n M;; inv_pexp (Exp (Rev x);; QFT x);; negator0 n x.
+   (Rev x); QFT x; rz_sub x n M; inv_exp ( (Rev x); QFT x); negator0 n x.
 
 (* Implementing x < y comparator. *)
 Definition rz_full_comparator (x:var) (n:nat) (c:posi) (y:var) := 
-    Exp (Rev x; Rev y);; QFT x;; QFT y;; Exp (rz_full_sub x n y);; RQFT x ;; Exp (CNOT (x,0) c);;
-    inv_pexp (Exp (Rev x; Rev y);; QFT x;; QFT y;; Exp (rz_full_sub x n y);; RQFT x).
+     (Rev x; Rev y); QFT x; QFT y; (rz_full_sub x n y); RQFT x ;  (CNOT (x,0) c);
+    inv_exp ( (Rev x; Rev y); QFT x; QFT y;  (rz_full_sub x n y); RQFT x).
 
 (* compare x < M *)
 Definition rz_compare_half3 (x:var) (n:nat) (c:posi) (M:nat -> bool) := 
-  Exp (rz_sub x n M) ;; RQFT x ;; Exp (CNOT (x,0) c).
+   (rz_sub x n M) ; RQFT x ; (CNOT (x,0) c).
 
 (* compare x >= M *)
 Definition rz_compare_half2 (x:var) (n:nat) (c:posi) (M:nat -> bool) := 
-  Exp (rz_sub x n M) ;; RQFT x ;; Exp (X (x,0); CNOT (x,0) c ; X (x,0)).
+   (rz_sub x n M) ; RQFT x ;  (X (x,0); CNOT (x,0) c ; X (x,0)).
 
 (* if x >= M, then the effect of x states. at this point, high-bit of x is 0. 
     otherwise, clean up x, and move on. *)
 Fixpoint rz_moder' i (n:nat) (x ex:var) (M:nat -> bool) := 
-     match i with 0 => Exp (SKIP (x,0))
-           | S j => rz_compare_half3 x n (ex,j) M ;; QFT x;;
-                     Exp (CU (ex,j) ((rz_adder x n M)));;
-                     Exp (X (ex,j));;
+     match i with 0 =>  (SKIP (x,0))
+           | S j => rz_compare_half3 x n (ex,j) M ; QFT x;
+                      (CU (ex,j) ((rz_adder x n M)));
+                      (X (ex,j));
                        rz_moder' j n x ex (cut_n (div_two_spec M) n)
      end.
 
 (* x % M circuit. *)
 Definition rz_moder (n:nat) (x re ex:var) (M:nat) := 
     let i := findnum M n in 
-        Exp (Rev x; Rev re);; QFT x;;
+         (Rev x; Rev re); QFT x;
           rz_moder' (S i) n x ex (nat2fb (2^i * M))
-            ;; (Exp (copyto x re n));; inv_pexp (rz_moder' (S i) n x ex (nat2fb (2^i * M)));;
-        inv_pexp (Exp (Rev x; Rev re);; QFT x).
+            ;( (copyto x re n)); inv_exp (rz_moder' (S i) n x ex (nat2fb (2^i * M)));
+        inv_exp ( (Rev x; Rev re); QFT x).
 
 Definition vars_for_rz_moder (size:nat) := 
   gen_vars (S size) (x_var::(y_var::(z_var::([])))).
@@ -3126,10 +2701,10 @@ Definition rz_moder_out (size:nat) :=
 (* x / M  circuit. *)
 Definition rz_div (n:nat) (x re ex:var) (M:nat) := 
     let i := findnum M n in 
-        Exp (Rev x);; QFT x;;
-         rz_moder' (S i) n x ex (nat2fb (2^i * M)) ;;
-           Exp (copyto ex re n);; inv_pexp (rz_moder' (S i) n x ex (nat2fb (2^i * M)));;
-        inv_pexp (Exp (Rev x);; QFT x).
+         (Rev x); QFT x;
+         rz_moder' (S i) n x ex (nat2fb (2^i * M)) ;
+            (copyto ex re n); inv_exp (rz_moder' (S i) n x ex (nat2fb (2^i * M)));
+        inv_exp ( (Rev x); QFT x).
 
 Definition vars_for_rz_div (size:nat) := 
   gen_vars size (x_var::(y_var::(z_var::([])))).
@@ -3143,9 +2718,9 @@ Definition rz_div_out (size:nat) :=
 (* x = (x % M, x / M)  circuit. *)
 Definition rz_div_mod (n:nat) (x ex:var) (M:nat) := 
     let i := findnum M (n-1) in 
-        Exp (Rev x);; QFT x;;
-            rz_moder' (S i) n x ex (nat2fb (2^i * M));;
-        inv_pexp (Exp (Rev x);; QFT x).
+         (Rev x); QFT x;
+            rz_moder' (S i) n x ex (nat2fb (2^i * M));
+        inv_exp ( (Rev x); QFT x).
 
 Definition vars_for_rz_div_mod (size:nat) := 
   gen_vars (S size) (x_var::(y_var::(([])))).
